@prefix : <https://w3id.org/pmd/mo/> .
@prefix owl: <http://www.w3.org/2002/07/owl#> .
@prefix rdf: <http://www.w3.org/1999/02/22-rdf-syntax-ns#> .
@prefix xml: <http://www.w3.org/XML/1998/namespace> .
@prefix xsd: <http://www.w3.org/2001/XMLSchema#> .
@prefix rdfs: <http://www.w3.org/2000/01/rdf-schema#> .
@base <https://w3id.org/pmd/co/2.0.7> .

<https://w3id.org/pmd/co/2.0.7> rdf:type owl:Ontology ;
                                 owl:versionIRI <https://w3id.org/pmd/mo/1.0.0> ;
                                 owl:imports <https://w3id.org/pmd/co/2.0.7> ;
                                 <http://purl.org/dc/elements/1.1/creator> <https://orcid.org/0000-0002-3717-7104> ,
                                                                           <https://orcid.org/0000-0002-7094-5371> ;
                                 <http://purl.org/dc/elements/1.1/license> <http://creativecommons.org/licenses/by/4.0> ;
                                 <http://purl.org/dc/terms/bibliographicCitation> "Markus Schilling, Bernd Bayerlein, June Lau. (January 29th, 2024) MO: microscopy ontology. Version 1.0.0, https://w3id.org/pmd/mo/"@en ;
                                 <http://purl.org/dc/terms/title> "Microscopy Ontology (MO)"@en ;
                                 rdfs:isDefinedBy <https://w3id.org/pmd/mo> ;
                                 <http://www.w3.org/2004/02/skos/core#definition> """Die Mikroskopie-Ontologie (MO) ist ein umfassender Rahmen für die Darstellung von Wissen, der Konzepte aus den Bereichen Mikroskopie und Mikroanalyse umfasst. Die MO basiert semantisch auf der PMD-Kernontologie PMDco (die in MO importiert wird), um eine Verbindung zu anderen MSE-Anwendungsontologien und domänenneutralen Konzepten in etablierten Top-Level-Ontologien zu ermöglichen. Das Hauptziel von MO ist es, ein standardisiertes Vokabular und einen Rahmen für die Beschreibung und Organisation von Konzepten, Entitäten und Beziehungen im Bereich der Mikroskopie und Mikroanalyse bereitzustellen. Diese Standardisierung erleichtert die Kommunikation und Interoperabilität zwischen verschiedenen Systemen, Datenbanken und Forschungsgruppen. Um ein Vokabular zu erhalten, das in diesem Bereich relevant und daher standardisierungswürdig ist, wurde ein NLP-Ansatz angewandt, mit dessen Hilfe häufig verwendete Begriffe ermittelt wurden. Auf der Grundlage dieser Liste von Begriffen wurde dann die MO entwickelt. In der Mikroskopie und Mikroanalytik fallen große Datenmengen aus verschiedenen Techniken und Instrumenten an. Die MO kann dazu beitragen, heterogene Datenquellen zu integrieren und zu verknüpfen, so dass Daten aus verschiedenen Experimenten und Studien effektiver kombiniert und analysiert werden können.
Darüber hinaus dient die MO als Grundlage für die Annotation von Mikroskopie- und Mikroanalysedaten mit standardisierten Metadaten. Diese erweiterte Metadatenbeschreibung verbessert die Interpretierbarkeit, Durchsuchbarkeit und Wiederverwendbarkeit von Daten und fördert die Transparenz und Reproduzierbarkeit in der Forschung. Darüber hinaus kann die MO durch die Formalisierung des Wissens über Instrumente, Techniken, Materialien und Phänomene die Grundlage für maschinelles Denken zur Unterstützung der Dateninterpretation, Hypothesenbildung und Versuchsplanung bilden.
Insgesamt soll MO die Forschung voranbringen, die Zusammenarbeit fördern und den Wissensaustausch in diesem interdisziplinären Bereich erleichtern."""@de ,
                                                                                  """The Microscopy Ontology (MO) is a comprehensive framework for representing knowledge that encompasses concepts from the domains of microscopy and microanalysis. The MO is semantically based on the mid-level PMD Core Ontology PMDco (which is imported in MO) to allow a connection to other MSE application ontologies and domain neutral concepts found in established top-level ontologies. The primary goal of MO is to provide a standardized vocabulary and framework for describing and organizing concepts, entities, and relationships within the field of microscopy and microanalysis. This standardization facilitates communication and interoperability between different systems, databases, and research groups. In order to obtain a vocabulary that is relevant in the field and therefore worth standardizing, an NLP approach was applied, with the help of which commonly used terms were determined. MO was then developed based on the respective list of terms. Microscopy and microanalysis generate vast amounts of data from various techniques and instruments. MO may help to integrate and link heterogeneous data sources, enabling the combination and analysis of data from different experiments and studies more effectively. Furthermore, MO serves as a basis for annotating microscopy and microanalysis data with standardized metadata. This improved metadata description enhances the interpretability, searchability, and reusability of data, promoting transparency and reproducibility in research. Moreover, by formalizing knowledge about instruments, techniques, materials, and phenomena, MO may provide the basis to enable machine reasoning to support data interpretation, hypothesis generation, and experimental design.
Overall, MO is intended to advance research, promoting collaboration, and facilitating knowledge exchange in this interdisciplinary domain."""@en .

#################################################################
#    Annotation properties
#################################################################

###  https://w3id.org/pmd/co/abbreviation
<https://w3id.org/pmd/co/abbreviation> rdf:type owl:AnnotationProperty .


###  https://w3id.org/pmd/mo/abbreviation
:abbreviation rdf:type owl:AnnotationProperty .


#################################################################
#    Classes
#################################################################

###  https://w3id.org/pmd/mo/Aberration
:Aberration rdf:type owl:Class ;
            rdfs:subClassOf <https://w3id.org/pmd/co/ValueObject> ;
            rdfs:isDefinedBy <https://w3id.org/pmd/mo> ;
            rdfs:label "Aberration"@de ,
                       "Aberration"@en ;
            <http://www.w3.org/2004/02/skos/core#definition> "Abweichung vom idealen oder erwarteten Verhalten, häufig im Zusammenhang mit optischen Systemen verwendet."@de ,
                                                             "Deviation from the ideal or expected behavior, often used in the context of optical systems."@en ;
            <https://w3id.org/pmd/co/definitionSource> "ChatGPT 3.5"@en .


###  https://w3id.org/pmd/mo/AccelerationVoltage
:AccelerationVoltage rdf:type owl:Class ;
                     rdfs:subClassOf :Voltage ;
                     rdfs:comment "Die Beschleunigungsspannung führt den Teilchen des Strahls kinetische Energie zu."@de ,
                                  "The acceleration voltage adds kinetic energy to the particles of the beam."@en ;
                     rdfs:isDefinedBy <https://w3id.org/pmd/mo> ;
                     rdfs:label "Acceleration Voltage"@en ,
                                "Beschleunigungsspannung"@de ;
                     <http://www.w3.org/2004/02/skos/core#definition> "Die Potentialdifferenz zwischen Anode und Kathode."@de ,
                                                                      "The potential difference between anode and cathode."@en ;
                     <https://w3id.org/pmd/co/definitionSource> <https://codebase.helmholtz.cloud/em_glossary/em_glossary/-/blob/main/terms/acceleration_voltage.yaml> .


###  https://w3id.org/pmd/mo/Angle
:Angle rdf:type owl:Class ;
       rdfs:subClassOf <https://w3id.org/pmd/co/ValueObject> ;
       rdfs:label <https://w3id.org/pmd/mo> ,
                  "Angle"@en ,
                  "Winkel"@de ;
       <http://www.w3.org/2004/02/skos/core#definition> """In der Geometrie und Trigonometrie ist ein Winkel ein Maß für eine Drehung, das erforderlich ist, um eine Linie oder Ebene mit einer anderen zur Deckung zu bringen. Ein Winkel wird durch zwei Strahlen gebildet, die einen gemeinsamen Endpunkt haben, der als Scheitelpunkt des Winkels bezeichnet wird. Die Strahlen werden als die Seiten des Winkels bezeichnet. 

Hinweis: Das Konzept des Winkels ist in der Geometrie von grundlegender Bedeutung und wird häufig verwendet, um die relative Ausrichtung von Linien, Ebenen oder Flächen zu beschreiben. Winkel werden in der Regel in Grad (°) oder Bogenmaß (rad) gemessen."""@de ,
                                                        """In geometry and trigonometry, an angle is a measure of the amount of rotation needed to bring one line or plane into coincidence with another. An angle is formed by two rays that share a common endpoint, known as the vertex of the angle. The rays are referred to as the sides of the angle. 

Note: The concept of an angle is fundamental in geometry and is often used to describe the relative orientation of lines, planes, or surfaces. Angles are typically measured in degrees (°) or radians (rad)."""@en ;
       <https://w3id.org/pmd/co/definitionSource> "ChatGPT 3.5"@en .


###  https://w3id.org/pmd/mo/AnnularBrightFieldScanningTransmissionElectronMicroscopy
:AnnularBrightFieldScanningTransmissionElectronMicroscopy rdf:type owl:Class ;
                                                          rdfs:subClassOf :ScanningTransmissionElectronMicroscopy ;
                                                          rdfs:isDefinedBy <https://w3id.org/pmd/mo> ;
                                                          rdfs:label "Annular Bright Field Scanning Transmission Electron Microscopy"@en ,
                                                                     "Ringförmige Hellfeld-Rastertransmissionselektronenmikroskopie"@de ;
                                                          <http://www.w3.org/2004/02/skos/core#definition> "ABF STEM is a technique that utilizes a specific arrangement of detectors to enhance contrast in STEM images, particularly for heavy elements."@en ;
                                                          <https://w3id.org/pmd/co/definitionSource> "ChatGPT 3.5"@en ;
                                                          :abbreviation "ABF-STEM"@en .


###  https://w3id.org/pmd/mo/AnnularDarkFieldScanningTransmissionElectronMicroscopy
:AnnularDarkFieldScanningTransmissionElectronMicroscopy rdf:type owl:Class ;
                                                        rdfs:subClassOf :ScanningTransmissionElectronMicroscopy ;
                                                        rdfs:isDefinedBy <https://w3id.org/pmd/mo> ;
                                                        rdfs:label "Annular Dark Field Scanning Transmission Electron Microscopy"@en ,
                                                                   "Ringförmige Dunkelfeld-Rastertransmissionselektronenmikroskopie"@de ;
                                                        <http://www.w3.org/2004/02/skos/core#definition> "ADF STEM is a technique that utilizes a specific arrangement of detectors to create contrast in STEM images based on the scattered electrons."@en ;
                                                        <https://w3id.org/pmd/co/definitionSource> "ChatGPT 3.5"@en ;
                                                        :abbreviation "ADF-STEM"@en .


###  https://w3id.org/pmd/mo/Anode
:Anode rdf:type owl:Class ;
       rdfs:subClassOf :Electrode ;
       rdfs:isDefinedBy <https://w3id.org/pmd/mo> ;
       rdfs:label "Anode"@de ,
                  "Anode"@en ;
       <http://www.w3.org/2004/02/skos/core#definition> "The anode is the positively charged electrode in an electrochemical cell or other electrically driven systems. It serves as the site where oxidation occurs, meaning electrons are released from the anode, typically moving towards the cathode. In devices like batteries, the anode is where electrons are produced during the discharge process."@en ;
       <https://w3id.org/pmd/co/definitionSource> "ChatGPT 3.5"@en .


###  https://w3id.org/pmd/mo/AtmosphericScanningElectronMicroscopy
:AtmosphericScanningElectronMicroscopy rdf:type owl:Class ;
                                       rdfs:subClassOf :ScanningElectronMicroscopy ;
                                       rdfs:isDefinedBy <https://w3id.org/pmd/mo> ;
                                       rdfs:label "Atmospheric Scanning Electron Microscopy"@en ,
                                                  "Atmosphärische Rasterelektronenmikroskopie"@de ;
                                       <http://www.w3.org/2004/02/skos/core#definition> "Atmospheric Scanning Electron Microscopy is a technique that allows samples to be imaged in their natural, hydrated state at atmospheric pressure. It enables the observation of biological and other hydrated specimens without the need for dehydration or coating."@en ;
                                       <https://w3id.org/pmd/co/definitionSource> "ChatGPT 3.5"@en ;
                                       :abbreviation "ASEM"@en .


###  https://w3id.org/pmd/mo/AtomicResolution
:AtomicResolution rdf:type owl:Class ;
                  rdfs:subClassOf :Resolution ;
                  rdfs:isDefinedBy <https://w3id.org/pmd/mo> ;
                  rdfs:label "Atomare Auflösung"@de ,
                             "Atomic Resolution"@en ;
                  <http://www.w3.org/2004/02/skos/core#definition> "Die Fähigkeit, einzelne Atome in einem Bild oder einer Struktur aufzulösen."@de ,
                                                                   "The ability to resolve individual atoms in an image or structure."@en ;
                  <https://w3id.org/pmd/co/definitionSource> "ChatGPT 3.5"@en .


###  https://w3id.org/pmd/mo/AugerElectronSpectroscopy
:AugerElectronSpectroscopy rdf:type owl:Class ;
                           rdfs:subClassOf :Spectroscopy ;
                           rdfs:isDefinedBy <https://w3id.org/pmd/mo> ;
                           rdfs:label "Auger Electron Spectroscopy"@en ,
                                      "Auger-Elektronen-Spektroskopie"@de ;
                           <http://www.w3.org/2004/02/skos/core#definition> """Auger Electron Spectroscopy (AES) is a surface analysis technique used in the field of materials science and surface chemistry. It involves the study of the interactions between high-energy electrons and atoms on the surface of a material. The process is named after Pierre Auger, who made significant contributions to the understanding of this phenomenon.
In AES, a sample's surface is bombarded with a beam of high-energy electrons, which causes inner-shell electrons to be ejected from the atoms in the sample. These vacancies are then filled by higher-energy electrons from outer shells, leading to the emission of Auger electrons. The energy of these emitted Auger electrons is characteristic of the specific elements present in the sample and their chemical states.
By analyzing the energy spectrum of the emitted Auger electrons, researchers can identify the elements present on the surface of the material and determine their relative concentrations. Auger Electron Spectroscopy provides valuable information about the elemental composition and chemical bonding of the top few atomic layers of a material, making it a powerful tool for studying surface properties, thin films, and interfaces in various scientific and industrial applications."""@en ;
                           <https://w3id.org/pmd/co/definitionSource> "ChatGPT 3.5"@en ;
                           :abbreviation "AES"@en .


###  https://w3id.org/pmd/mo/Beam
:Beam rdf:type owl:Class ;
      rdfs:subClassOf <https://w3id.org/pmd/co/Object> ;
      rdfs:comment "In an electron microscope particles are originally emitted by an  particle source and intended to interact with a sample or a detector. The definition here should be differentiated from particles moving due to electrochemical gradient (i.e. in diffusion of liquids). Due to the wave-particle duality, a beam can also be  considered as a series of waves propagating in a common direction."@en ,
                   "In einem Elektronenmikroskop werden Teilchen ursprünglich von einer Teilchenquelle emittiert und sollen mit einer Probe oder einem Detektor wechselwirken. Die Definition sollte hier von Teilchen unterschieden werden, die sich aufgrund eines elektrochemischen Gradienten bewegen (z. B. bei der Diffusion von Flüssigkeiten). Aufgrund des Welle-Teilchen-Dualismus kann ein Strahl auch als eine Reihe von Wellen betrachtet werden, die sich in einer gemeinsamen Richtung ausbreiten."@de ;
      rdfs:isDefinedBy <https://w3id.org/pmd/mo> ;
      rdfs:label "Beam"@en ,
                 "Strahl"@de ;
      <http://www.w3.org/2004/02/skos/core#altLabel> "Strahl geladener Teilchen"@de ,
                                                     "charged particle beam"@en ;
      <http://www.w3.org/2004/02/skos/core#definition> "A group of particles which move, on average, in a common direction."@en ,
                                                       "Eine Gruppe von Teilchen, die sich im Durchschnitt in eine gemeinsame Richtung bewegen."@de ;
      <https://w3id.org/pmd/co/definitionSource> <https://codebase.helmholtz.cloud/em_glossary/em_glossary/-/blob/main/terms/beam.yaml> .


###  https://w3id.org/pmd/mo/BeamCurrent
:BeamCurrent rdf:type owl:Class ;
             rdfs:subClassOf :Current ;
             rdfs:comment "Der Wert des Strahlstroms variiert entlang der Strahlachse. Die Punkte, an denen der Strahlstrom gemessen wird, sind je nach Gerät und Hersteller unterschiedlich. Der Strahlstrom wird immer in Bezug auf die Erde gemessen."@de ,
                          "The value of beam current varies along the beam axis. The points  at which the beam current is measured varies between instruments and manufacturers. Beam current is always measured with respect to ground."@en ;
             rdfs:isDefinedBy <https://w3id.org/pmd/mo> ;
             rdfs:label "Beam Current"@en ,
                        "Strahlungsstrom"@de ;
             <http://www.w3.org/2004/02/skos/core#definition> "Electrical current which flows along the beam path."@en ,
                                                              "Elektrischer Strom, der entlang des Strahlengangs fließt."@de ;
             <https://w3id.org/pmd/co/definitionSource> <https://codebase.helmholtz.cloud/em_glossary/em_glossary/-/blob/main/terms/beam_current.yaml> .


###  https://w3id.org/pmd/mo/BeamEnergy
:BeamEnergy rdf:type owl:Class ;
            rdfs:subClassOf :Energy ;
            rdfs:isDefinedBy <https://w3id.org/pmd/mo> ;
            rdfs:label "Beam Energy"@en ,
                       "Strahlungsenergie"@de ;
            <http://www.w3.org/2004/02/skos/core#definition> "Die Energie eines Teilchen- oder Photonenstrahls, der in verschiedenen Analyseverfahren verwendet wird."@de ,
                                                             "The energy of a particle or photon beam used in various analytical techniques."@en ;
            <https://w3id.org/pmd/co/definitionSource> "ChatGPT 3.5"@en .


###  https://w3id.org/pmd/mo/BeamPath
:BeamPath rdf:type owl:Class ;
          rdfs:subClassOf <https://w3id.org/pmd/co/Object> ;
          rdfs:isDefinedBy <https://w3id.org/pmd/mo> ;
          rdfs:label "Beam Path"@en ,
                     "Strahlengang"@de ;
          <http://www.w3.org/2004/02/skos/core#altLabel> "Strahlenweg"@de ;
          <http://www.w3.org/2004/02/skos/core#definition> "Path which the beam flows along defined by the optical components of the instrument."@en ,
                                                           "Pfad, den der Strahl entlangfließt und der durch die optischen Komponenten des Geräts definiert ist."@de ;
          <https://w3id.org/pmd/co/definitionSource> <https://codebase.helmholtz.cloud/em_glossary/em_glossary/-/blob/main/terms/beam_path.yaml> .


###  https://w3id.org/pmd/mo/BrightFieldTransmissionElectronMicroscopy
:BrightFieldTransmissionElectronMicroscopy rdf:type owl:Class ;
                                           rdfs:subClassOf :TransmissionElectronMicroscopy ;
                                           rdfs:isDefinedBy <https://w3id.org/pmd/mo> ;
                                           rdfs:label "Bright Field Transmission Electron Microscopy"@en ,
                                                      "Hellfeld-Transmissionselektronenmikroskopie"@de ;
                                           <http://www.w3.org/2004/02/skos/core#definition> "Bright Field TEM is an imaging mode in transmission electron microscopy where regions of the sample that scatter electrons less appear brighter in the resulting image."@en ;
                                           <https://w3id.org/pmd/co/definitionSource> "ChatGPT 3.5"@en ;
                                           :abbreviation "BFTEM"@en .


###  https://w3id.org/pmd/mo/CameraLength
:CameraLength rdf:type owl:Class ;
              rdfs:subClassOf <https://w3id.org/pmd/co/Length> ;
              rdfs:comment "Diese Definition gilt für die experimentelle Technik der Fraunhofer-Fernfeldbeugung. Im Beugungsmodus wird die Größe Kameralänge verwendet, um den Grad der Vergrößerung des Beugungsmusters auf dem Detektor zu bestimmen. Man beachte, dass die Kameralänge durch das Hinzufügen von Linsen im Strahl verändert werden kann, wodurch die physikalische Größe in eine virtuelle Größe umgewandelt wird. Ursprünglich wurde der Begriff Kameralänge im TEM verwendet, in jüngster Zeit gibt es jedoch auch innovative Anwendungen im REM (siehe Beispiele). Die Kameralänge hängt vom optischen Aufbau ab und wird idealerweise durch Kalibrierungsmessungen mit bekannten Proben, z. B. Gold auf Kohlenstoff, bestimmt."@de ,
                           "This definition applies to the experimental technique of Fraunhofer far field diffraction.  In diffraction mode the quantity camera length is used to qualify the level of magnification of  the diffraction pattern onto the detector. Note that the camera length may by altered by the addition of lenses in the beam transforming the physical quantity in a virtual one. Historically the term camera length was used in TEM, however more recently there have been innovative applications in SEM, see examples. Camera length depends on the optical setup and it is ideally determined from calibration measurements using known samples, e.g., gold on carbon."@en ;
              rdfs:isDefinedBy <https://w3id.org/pmd/mo> ;
              <http://www.w3.org/2004/02/skos/core#definition> "Abstand, der zwischen der Probenoberfläche und der Detektorebene besteht."@de ,
                                                               "Distance which is present between the specimen surface and the detector plane."@en ;
              <http://www.w3.org/2004/02/skos/core#example> <https://doi.org/10.1016/j.ultramic.2020.112956> ,
                                                            <https://doi.org/10.1017/S1431927619002988> ;
              <https://w3id.org/pmd/co/definitionSource> <https://codebase.helmholtz.cloud/em_glossary/em_glossary/-/blob/main/terms/camera_length.yaml> ,
                                                         "Camera Length"@en ,
                                                         "Kameralänge"@de .


###  https://w3id.org/pmd/mo/Cathode
:Cathode rdf:type owl:Class ;
         rdfs:subClassOf :Electrode ;
         rdfs:isDefinedBy <https://w3id.org/pmd/mo> ;
         rdfs:label "Cathode"@en ,
                    "Kathode"@de ;
         <http://www.w3.org/2004/02/skos/core#definition> "The cathode is the negatively charged electrode in an electrochemical cell or other electrical systems. It is the site where reduction occurs, leading to the acceptance of electrons from the external circuit. In batteries, for instance, the cathode is where electrons are consumed during the discharge process."@en ;
         <https://w3id.org/pmd/co/definitionSource> "ChatGPT 3.5"@en .


###  https://w3id.org/pmd/mo/ChromaticAberration
:ChromaticAberration rdf:type owl:Class ;
                     rdfs:subClassOf :Aberration ;
                     rdfs:isDefinedBy <https://w3id.org/pmd/mo> ;
                     rdfs:label "Chromatic Aberration"@en ,
                                "Chromatische Aberration"@de ;
                     <http://www.w3.org/2004/02/skos/core#definition> "Die Unfähigkeit eines Objektivs, alle Farben auf denselben Konvergenzpunkt zu fokussieren."@de ,
                                                                      "The failure of a lens to focus all colors to the same convergence point."@en ;
                     <https://w3id.org/pmd/co/definitionSource> "ChatGPT 3.5"@en .


###  https://w3id.org/pmd/mo/CoherentBeam
:CoherentBeam rdf:type owl:Class ;
              rdfs:subClassOf :Beam ;
              rdfs:comment "In dieser Definition beziehen wir uns auf Teilwellen."@de ,
                           "In this definition we refer to partial waves."@en ;
              rdfs:isDefinedBy <https://w3id.org/pmd/mo> ;
              rdfs:label "Coherent Beam"@en ,
                         "Kohärenter Strahl"@de ;
              <http://www.w3.org/2004/02/skos/core#definition> "A monochromatic beam which consists of waves that have a defined phase relationship."@en ,
                                                               "Ein monochromatischer Strahl, der aus Wellen besteht, die eine bestimmte Phasenbeziehung haben."@de ;
              <https://w3id.org/pmd/co/definitionSource> <https://codebase.helmholtz.cloud/em_glossary/em_glossary/-/blob/main/terms/coherent_beam.yaml> .


###  https://w3id.org/pmd/mo/CollectionEfficiency
:CollectionEfficiency rdf:type owl:Class ;
                      rdfs:subClassOf :Efficiency ;
                      rdfs:isDefinedBy <https://w3id.org/pmd/mo> ;
                      rdfs:label "Collection Efficiency"@en ,
                                 "Kollektoreffizienz"@de ;
                      <http://www.w3.org/2004/02/skos/core#definition> "Die Fähigkeit eines Detektors oder Systems, relevante Signale oder Daten zu erfassen und aufzuzeichnen."@de ,
                                                                       "The ability of a detector or system to capture and record relevant signals or data."@en ;
                      <https://w3id.org/pmd/co/definitionSource> "ChatGPT 3.5"@en .


###  https://w3id.org/pmd/mo/CondensorLense
:CondensorLense rdf:type owl:Class ;
                rdfs:subClassOf <https://w3id.org/pmd/co/ProcessingNode> ;
                rdfs:isDefinedBy <https://w3id.org/pmd/mo> ;
                rdfs:label "Condensor Lense"@en ,
                           "Kondensorlinse"@de ;
                <http://www.w3.org/2004/02/skos/core#definition> "A condenser lens is an optical element used in microscopy and other optical systems to focus and control the illumination on the sample being observed. It is positioned below the light source and directs light rays onto the specimen, making the illumination uniform and optimizing the quality of the sample's image. The condenser lens helps enhance contrast, resolution, and overall image quality by ensuring that a consistent and concentrated light beam illuminates the specimen."@en ;
                <https://w3id.org/pmd/co/definitionSource> "ChatGPT 3.5"@en .


###  https://w3id.org/pmd/mo/ConfocalLaserScanningMicroscopy
:ConfocalLaserScanningMicroscopy rdf:type owl:Class ;
                                 rdfs:subClassOf :LightMicroscopy ;
                                 rdfs:isDefinedBy <https://w3id.org/pmd/mo> ;
                                 rdfs:label "Confocal Laser Scanning Microscopy"@en ,
                                            "Konfokale Laser-Scanning-Mikroskopie"@de ;
                                 <http://www.w3.org/2004/02/skos/core#definition> "Confocal Laser Scanning Microscopy (CLSM) is an optical imaging technique that enhances resolution and eliminates out-of-focus blur by using a spatial pinhole and laser illumination. A focused laser beam is scanned across the sample's surface or depth, and only the light emitted from the focal plane (or a defined section) passes through the pinhole to form an image. CLSM provides high-resolution three-dimensional images, making it popular for biological imaging and studying fluorescently labeled samples."@en ;
                                 <https://w3id.org/pmd/co/definitionSource> "ChatGPT 3.5"@en ;
                                 :abbreviation "CLSM"@en .


###  https://w3id.org/pmd/mo/ConvergenceAngle
:ConvergenceAngle rdf:type owl:Class ;
                  rdfs:subClassOf :Angle ;
                  rdfs:comment "Der Konvergenzwinkel eines Strahls ist sowohl im REM als auch im TEM von großer Bedeutung, da er sich auf eine Vielzahl von Bildeigenschaften auswirkt. Er wird durch die Fokussierungsstärke der strahlformenden Linse beeinflusst und kann durch Einfügen von Blenden in den Strahlengang verringert werden."@de ,
                               "The convergence angle of a beam is of high relevance in both SEM and TEM as it impacts a variety of image properties. It is affected by the focusing strength of the beam forming lens and can be reduced by inserting apertures into the beam path."@en ;
                  rdfs:isDefinedBy <https://w3id.org/pmd/mo> ;
                  rdfs:label "Convergence Angle"@en ,
                             "Konvergenzwinkel"@de ;
                  <http://www.w3.org/2004/02/skos/core#definition> "Der Winkel, der durch den Halböffnungswinkel des Kegels bei einem konvergenten Strahl gegeben ist."@de ,
                                                                   "The angle which is given by the semi-opening angle of the cone in a convergent beam."@en ;
                  <https://w3id.org/pmd/co/definitionSource> <https://codebase.helmholtz.cloud/em_glossary/em_glossary/-/blob/main/terms/convergence_angle.yaml> .


###  https://w3id.org/pmd/mo/Cryo-ScanningElectronMicroscope
:Cryo-ScanningElectronMicroscope rdf:type owl:Class ;
                                 rdfs:subClassOf :ScanningElectronMicroscope ;
                                 rdfs:comment "A cryo-scanning electron microscope is typically used for imaging biological samples."@en ,
                                              "Ein Kryo-Rasterelektronenmikroskop wird in der Regel zur Abbildung biologischer Proben verwendet."@de ,
                                              "Eine Art Elektronenmikroskop, das bei kryogenen Temperaturen arbeitet."@de ;
                                 rdfs:isDefinedBy <https://w3id.org/pmd/mo> ;
                                 rdfs:label "Cryo Scanning Electron Microscope"@en ,
                                            "Kryo-Rasterelektronenmikroskop"@de ,
                                            "cryo-SEM"@en ;
                                 <http://www.w3.org/2004/02/skos/core#definition> "A type of electron microscope that operates under cryogenic temperatures."@en ;
                                 <https://w3id.org/pmd/co/definitionSource> "ChatGPT 3.5"@en .


###  https://w3id.org/pmd/mo/CryoElectronTomography
:CryoElectronTomography rdf:type owl:Class ;
                        rdfs:subClassOf :ElectronTomography ;
                        rdfs:isDefinedBy <https://w3id.org/pmd/mo> ;
                        rdfs:label "Cryo Electron Tomography"@en ,
                                   "Kryo-Elektronentomographie"@de ;
                        <http://www.w3.org/2004/02/skos/core#definition> "Cryo Electron Tomography is a form of electron tomography that is performed at cryogenic temperatures. It is used to study the three-dimensional structure of frozen-hydrated samples."@en ;
                        <https://w3id.org/pmd/co/definitionSource> "ChatGPT 3.5"@en ;
                        :abbreviation "cryo-ET"@en .


###  https://w3id.org/pmd/mo/CryoTransmissionElectronMicroscope
:CryoTransmissionElectronMicroscope rdf:type owl:Class ;
                                    rdfs:subClassOf :TransmissionElectronMicroscope ;
                                    rdfs:isDefinedBy <https://w3id.org/pmd/mo> ;
                                    rdfs:label "Cryo Transmission Electron Microscope"@en ,
                                               "Kryo-Transmissionselektronenmikroskop"@de ;
                                    <http://www.w3.org/2004/02/skos/core#definition> "A transmission electron microscope that operates at cryogenic temperatures."@en ,
                                                                                     "Ein Transmissionselektronenmikroskop, das bei kryogenen Temperaturen arbeitet."@de ;
                                    <https://w3id.org/pmd/co/definitionSource> "ChatGPT 3.5"@en ;
                                    :abbreviation "cryo-TEM"@en .


###  https://w3id.org/pmd/mo/Current
:Current rdf:type owl:Class ;
         rdfs:subClassOf <https://w3id.org/pmd/co/ValueObject> ;
         rdfs:comment "Der Strom wird normalerweise in Ampere (A) gemessen."@de ,
                      "The current is typically measured in amperes (A)."@en ;
         rdfs:isDefinedBy <https://w3id.org/pmd/mo> ;
         rdfs:label "Current"@en ,
                    "Strom"@de ;
         <http://www.w3.org/2004/02/skos/core#altLabel> "Stromstärke"@de ;
         <http://www.w3.org/2004/02/skos/core#definition> "Der Fluss der elektrischen Ladung."@de ,
                                                          "The flow of electric charge."@en ;
         <https://w3id.org/pmd/co/definitionSource> "ChatGPT 3.5"@en .


###  https://w3id.org/pmd/mo/DetectorQuantumEfficiency
:DetectorQuantumEfficiency rdf:type owl:Class ;
                           rdfs:subClassOf :Efficiency ;
                           rdfs:isDefinedBy <https://w3id.org/pmd/mo> ;
                           rdfs:label "Detector Quantum Efficiency"@en ,
                                      "Detektor Quantenausbeute"@de ;
                           <http://www.w3.org/2004/02/skos/core#definition> "Die Effizienz, mit der ein Detektor einfallende Strahlung in Nutzsignale umwandelt."@de ,
                                                                            "The efficiency with which a detector converts incident radiation into useful signals."@en ;
                           <https://w3id.org/pmd/co/definitionSource> "ChatGPT 3.5"@en .


###  https://w3id.org/pmd/mo/Diffraction
:Diffraction rdf:type owl:Class ;
             rdfs:subClassOf :PhysicalProcess ;
             rdfs:comment "Der in dieser Definition verwendete Begriff \"Materie\" bezieht sich sowohl auf kristalline als auch auf amorphe Materie (z. B. Gase oder Gegenstände)."@de ,
                          "The term \"matter\" used in this definition is meant to represent crystalline as well as amorphous matter (e.g. gases or objects)."@en ;
             rdfs:isDefinedBy <https://w3id.org/pmd/mo> ;
             rdfs:label "Diffraction"@en ,
                        "Diffraktion"@de ;
             <http://www.w3.org/2004/02/skos/core#altLabel> "Beugung"@de ,
                                                            "Scattering"@en ;
             <http://www.w3.org/2004/02/skos/core#definition> "A physical phenomenon during which the direction and intensity of a propagating wave is changed due to interaction with matter having structure dimensions in the order of the wavelength."@en ,
                                                              "Ein physikalisches Phänomen, bei dem sich die Richtung und Intensität einer sich ausbreitenden Welle aufgrund der Wechselwirkung mit Materie mit Strukturabmessungen in der Größenordnung der Wellenlänge ändert."@de ;
             <https://w3id.org/pmd/co/definitionSource> <https://codebase.helmholtz.cloud/em_glossary/em_glossary/-/blob/main/terms/diffraction.yaml> .


###  https://w3id.org/pmd/mo/DiffractionPattern
:DiffractionPattern rdf:type owl:Class ;
                    rdfs:subClassOf <https://w3id.org/pmd/co/DigitalEntity> ;
                    rdfs:comment "Aus praktischen Gründen unterscheiden wir hier nicht zwischen dem physikalischen Phänomen eines Beugungsmusters und der experimentellen Aufzeichnung eines Beugungsmusters, obwohl wir wissen, dass es sich dabei um zwei verschiedene Konzepte handelt. Ein Beugungsmuster wird in der Regel als Bild aufgezeichnet. Eine Änderung der Geometrie und/oder der Ausrichtung des Detektors hat einen direkten Einfluss auf das erfasste Muster."@de ,
                                 "For practical purposes we do not distinguish here between the physical phenomenon of a diffraction pattern, and the experimental recording of a diffraction pattern although we realize that these are indeed separate concepts. A diffraction pattern is commonly recorded  as an image. Changing the geometry and/or the orientation of the detector will directly influence the pattern detected."@en ;
                    rdfs:isDefinedBy <https://w3id.org/pmd/mo> ;
                    rdfs:label "Beugungsmuster"@de ,
                               "Diffraction Pattern"@en ;
                    <http://www.w3.org/2004/02/skos/core#definition> "A spatial intensity modulation which is generated by diffraction."@en ,
                                                                     "Eine räumliche Intensitätsmodulation, die durch Beugung erzeugt wird."@de ;
                    <https://w3id.org/pmd/co/definitionSource> <https://codebase.helmholtz.cloud/em_glossary/em_glossary/-/blob/main/terms/diffraction_pattern.yaml> .


###  https://w3id.org/pmd/mo/DiskOfLeastConfusion
:DiskOfLeastConfusion rdf:type owl:Class ;
                      rdfs:subClassOf <https://w3id.org/pmd/co/CrossSectionArea> ;
                      rdfs:isDefinedBy <https://w3id.org/pmd/mo> ;
                      rdfs:label "Disk Of Least Confusion"@en ,
                                 "Scheibe der geringsten Konfusion"@de ;
                      <http://www.w3.org/2004/02/skos/core#definition> "A cross section of a beam at which the beam has the smallest spatial extent."@en ,
                                                                       "Ein Querschnitt eines Strahls, an dem der Strahl die kleinste räumliche Ausdehnung hat."@de ;
                      <https://w3id.org/pmd/co/definitionSource> <https://codebase.helmholtz.cloud/em_glossary/em_glossary/-/blob/main/terms/disk_of_least_confusion.yaml> .


###  https://w3id.org/pmd/mo/DwellTime
:DwellTime rdf:type owl:Class ;
           rdfs:subClassOf <https://w3id.org/pmd/co/Duration> ;
           rdfs:isDefinedBy <https://w3id.org/pmd/mo> ;
           rdfs:label "Dwell Time"@en ,
                      "Verweilzeit"@de ;
           <http://www.w3.org/2004/02/skos/core#altLabel> "Verweildauer"@de ;
           <http://www.w3.org/2004/02/skos/core#definition> "Time period during which the beam remains at one position."@en ,
                                                            "Zeitspanne, in der der Strahl an einer Position bleibt."@de ;
           <https://w3id.org/pmd/co/definitionSource> <https://codebase.helmholtz.cloud/em_glossary/em_glossary/-/blob/main/terms/dwell_time.yaml> ,
                                                      <https://doi.org/10.1007/978-1-4939-6676-9> ,
                                                      <https://www.iso.org/obp/ui/#iso:std:iso:22493:ed-2:v1:en> .


###  https://w3id.org/pmd/mo/DynamicFocusCorrection
:DynamicFocusCorrection rdf:type owl:Class ;
                        rdfs:subClassOf <https://w3id.org/pmd/co/AnalysingProcess> ;
                        rdfs:comment "Relevant when an area is scanned which extends off-(tilt) axis. An option in a GUI to switch on. An automatic change of the electron optics to keep the sample in focus. Implementation strongly depends on the microscope and its control software. Information about dynamic focus correction may help others to understand the quality of an experiment."@en ,
                                     "Relevant, wenn ein Bereich gescannt wird, der sich außerhalb der (Neigungs-)Achse befindet. Eine Option in einer GUI zum Einschalten. Eine automatische Änderung der Elektronenoptik, um die Probe im Fokus zu halten. Die Implementierung hängt stark vom Mikroskop und dessen Steuerungssoftware ab. Informationen über die dynamische Fokuskorrektur können anderen helfen, die Qualität eines Experiments zu verstehen."@de ;
                        rdfs:isDefinedBy <https://w3id.org/pmd/mo> ;
                        rdfs:label "Dynamic Focus Correction"@en ,
                                   "Dynamische Fokuskorrektur"@de ;
                        <http://www.w3.org/2004/02/skos/core#definition> "Dynamic refocussing which keeps the electron probe focused on the surface of a tilted sample."@en ,
                                                                         "Dynamische Refokussierung, die die Elektronensonde auf der Oberfläche einer gekippten Probe fokussiert."@de ;
                        <https://w3id.org/pmd/co/definitionSource> <https://codebase.helmholtz.cloud/em_glossary/em_glossary/-/blob/main/terms/dynamic_focus_correction.yaml> .


###  https://w3id.org/pmd/mo/DynamicRefocusing
:DynamicRefocusing rdf:type owl:Class ;
                   rdfs:subClassOf <https://w3id.org/pmd/co/AnalysingProcess> ;
                   rdfs:comment "To achieve experimental reproducibility this workflow should be described in detail."@en ,
                                "Um die Reproduzierbarkeit der Versuche zu gewährleisten, sollte dieser Arbeitsablauf detailliert beschrieben werden."@de ;
                   rdfs:isDefinedBy <https://w3id.org/pmd/mo> ;
                   rdfs:label "Dynamic Refocusing"@en ,
                              "Dynamische Refokussierung"@de ;
                   <http://www.w3.org/2004/02/skos/core#altLabel> "Dynamische Neufokussierung"@de ;
                   <http://www.w3.org/2004/02/skos/core#definition> "A workflow to keep the specimen in focus by automatic means."@en ,
                                                                    "Ein Arbeitsablauf, bei dem die Probe automatisch fokussiert wird."@de ;
                   <https://w3id.org/pmd/co/definitionSource> <https://codebase.helmholtz.cloud/em_glossary/em_glossary/-/blob/main/terms/dynamic_refocusing.yaml> .


###  https://w3id.org/pmd/mo/DynamicTransmissionElectronMicroscopy
:DynamicTransmissionElectronMicroscopy rdf:type owl:Class ;
                                       rdfs:subClassOf :TransmissionElectronMicroscopy ;
                                       rdfs:isDefinedBy <https://w3id.org/pmd/mo> ;
                                       rdfs:label "Dynamic Transmission Electron Microscopy"@en ,
                                                  "Dynamische Transmissionselektronenmikroskopie"@de ;
                                       <http://www.w3.org/2004/02/skos/core#definition> "Dynamic Transmission Electron Microscopy is a technique that uses ultrafast electron pulses to capture rapid processes in materials with nanosecond to picosecond time resolution."@en ;
                                       <https://w3id.org/pmd/co/definitionSource> "ChatGPT 3.5"@en ;
                                       :abbreviation "DTEM"@en .


###  https://w3id.org/pmd/mo/Efficiency
:Efficiency rdf:type owl:Class ;
            rdfs:subClassOf <https://w3id.org/pmd/co/ValueObject> ;
            rdfs:isDefinedBy <https://w3id.org/pmd/mo> ;
            rdfs:label "Efficiency"@en ,
                       "Effizienz"@de ;
            <http://www.w3.org/2004/02/skos/core#definition> "Das Verhältnis von nützlichem / nutzbarem Output zum gesamten Input in einem System."@de ,
                                                             "The ratio of useful output to total input in any system."@en ;
            <https://w3id.org/pmd/co/definitionSource> "ChatGPT 3.5"@en .


###  https://w3id.org/pmd/mo/Electrode
:Electrode rdf:type owl:Class ;
           rdfs:subClassOf <https://w3id.org/pmd/co/ProcessingNode> ;
           rdfs:isDefinedBy <https://w3id.org/pmd/mo> ;
           rdfs:label "Electrode"@en ,
                      "Elektrode"@de ;
           <http://www.w3.org/2004/02/skos/core#definition> "An electrode is a conductor through which electric current enters or exits a substance. In the context of electrochemical systems, an electrode facilitates the transfer of electrons between a solid material and an electrolyte. Electrodes are essential components in batteries, fuel cells, electroplating, and other electrochemical processes. They play a critical role in facilitating chemical reactions and energy storage or conversion."@en ;
           <https://w3id.org/pmd/co/definitionSource> "ChatGPT 3.5"@en .


###  https://w3id.org/pmd/mo/ElectronBackscatterDiffraction
:ElectronBackscatterDiffraction rdf:type owl:Class ;
                                rdfs:subClassOf :ElectronDiffraction ;
                                rdfs:isDefinedBy <https://w3id.org/pmd/mo> ;
                                rdfs:label "Electron Backscatter Diffraction"@en ,
                                           "Rückstreuelektronenbeugung"@de ;
                                <http://www.w3.org/2004/02/skos/core#definition> "Electron Backscatter Diffraction is a microscopy technique used to analyze the crystallographic orientation and microstructure of materials. It involves directing an electron beam onto a sample's surface and measuring the backscattered electrons. By analyzing the diffraction patterns of these electrons, researchers can determine the crystallographic orientation of the material's grains."@en ;
                                <https://w3id.org/pmd/co/definitionSource> "ChatGPT 3.5"@en ;
                                :abbreviation "EBSD"@en .


###  https://w3id.org/pmd/mo/ElectronBeam
:ElectronBeam rdf:type owl:Class ;
              rdfs:subClassOf :Beam ;
              rdfs:isDefinedBy <https://w3id.org/pmd/mo> ;
              rdfs:label "Electron Beam"@en ,
                         "Elektronenstrahl"@de ;
              <http://www.w3.org/2004/02/skos/core#definition> "A beam which consists of electrons."@en ,
                                                               "Ein Strahl, der aus Elektronen besteht."@de ;
              <https://w3id.org/pmd/co/definitionSource> <https://codebase.helmholtz.cloud/em_glossary/em_glossary/-/blob/main/terms/electron_beam.yaml> .


###  https://w3id.org/pmd/mo/ElectronChannelingContrastImaging
:ElectronChannelingContrastImaging rdf:type owl:Class ;
                                   rdfs:subClassOf :ScanningElectronMicroscopy ;
                                   rdfs:isDefinedBy <https://w3id.org/pmd/mo> ;
                                   rdfs:label "Electron Channeling Contrast Imaging"@en ,
                                              "Elektronenkanal-Kontrastbildgebung"@de ;
                                   <http://www.w3.org/2004/02/skos/core#definition> "Electron Channeling Contrast Imaging is a technique used in SEM or TEM to study crystallographic defects, such as dislocations, in crystalline materials. It utilizes the contrast resulting from the deviation of electron trajectories due to crystal defects."@en ;
                                   <https://w3id.org/pmd/co/definitionSource> "ChatGPT 3.5"@en ;
                                   :abbreviation "ECCI"@en .


###  https://w3id.org/pmd/mo/ElectronDiffraction
:ElectronDiffraction rdf:type owl:Class ;
                     rdfs:subClassOf :Diffraction ;
                     rdfs:isDefinedBy <https://w3id.org/pmd/mo> ;
                     rdfs:label "Electron Diffraction"@en ,
                                "Elektronenbeugung"@de ;
                     <http://www.w3.org/2004/02/skos/core#definition> "Beugung, die auf einer sich ausbreitenden Elektronenwelle beruht."@de ,
                                                                      "Diffraction which is based on a propagating electron wave."@en ;
                     <https://w3id.org/pmd/co/definitionSource> <https://codebase.helmholtz.cloud/em_glossary/em_glossary/-/blob/main/terms/electron_diffraction.yaml> ,
                                                                <https://en.wikipedia.org/wiki/Diffraction> ,
                                                                <https://www.sciencedirect.com/topics/chemistry/electron-diffraction#:~:text=Electron%20diffraction%20is%20a%20technique,resulting%20in%20a%20diffraction%20pattern> .


###  https://w3id.org/pmd/mo/ElectronDiffractionPattern
:ElectronDiffractionPattern rdf:type owl:Class ;
                            rdfs:subClassOf :DiffractionPattern ;
                            rdfs:isDefinedBy <https://w3id.org/pmd/mo> ;
                            rdfs:label "Electron Diffraction Pattern"@en ,
                                       "Elektronenbeugungsmuster"@de ;
                            <http://www.w3.org/2004/02/skos/core#altLabel> "Elektronenbeugungsbild"@de ;
                            <http://www.w3.org/2004/02/skos/core#definition> "A diffraction pattern which is generated from electron diffraction."@en ,
                                                                             "Ein Beugungsmuster, das durch Elektronenbeugung erzeugt wird."@de ;
                            <https://w3id.org/pmd/co/definitionSource> <https://codebase.helmholtz.cloud/em_glossary/em_glossary/-/blob/main/terms/electron_diffraction_pattern.yaml> .


###  https://w3id.org/pmd/mo/ElectronEnergyLossSpectroscopy
:ElectronEnergyLossSpectroscopy rdf:type owl:Class ;
                                rdfs:subClassOf :Spectroscopy ;
                                rdfs:isDefinedBy <https://w3id.org/pmd/mo> ;
                                rdfs:label "Electron Energy Loss Spectroscopy"@en ,
                                           "Elektronenenergieverlustspektroskopie"@de ;
                                <http://www.w3.org/2004/02/skos/core#definition> """Electron Energy Loss Spectroscopy (EELS) is a specialized analytical technique in the field of materials science and electron microscopy. It involves the measurement of the energy loss of electrons as they interact with a sample. EELS is commonly performed in transmission electron microscopy (TEM) setups.
In EELS, a focused beam of high-energy electrons is directed at a sample. As these electrons pass through the material, they can lose energy through various interactions, such as inelastic scattering and excitation of inner-shell electrons. The energy loss is measured and analyzed to gain information about the sample's composition, electronic structure, and bonding characteristics.
By studying the energy loss spectrum, researchers can identify the types of atoms present in the sample, determine their chemical states, and gather insights into the electronic properties of the material. EELS is particularly useful for investigating nanoscale materials, thin films, and interfaces, providing valuable information about their electronic and atomic structure. It is a powerful technique for understanding the behavior of materials at the nanometer scale and plays a significant role in advancing fields such as materials science, nanotechnology, and semiconductor research."""@en ;
                                <https://w3id.org/pmd/co/definitionSource> "ChatGPT 3.5"@en ;
                                :abbreviation "EELS"@en .


###  https://w3id.org/pmd/mo/ElectronMicroprobe
:ElectronMicroprobe rdf:type owl:Class ;
                    rdfs:subClassOf <https://w3id.org/pmd/co/ElectronMicroscope> ;
                    rdfs:isDefinedBy <https://w3id.org/pmd/mo> ;
                    rdfs:label "Electron Microprobe"@en ,
                               "Elektronenmikrosonde"@de ;
                    <http://www.w3.org/2004/02/skos/core#definition> "An analytical instrument used to determine the chemical composition of materials."@en ,
                                                                     "Ein Analyseinstrument zur Bestimmung der chemischen Zusammensetzung von Materialien."@de ;
                    <https://w3id.org/pmd/co/definitionSource> "ChatGPT 3.5"@en .


###  https://w3id.org/pmd/mo/ElectronProbe
:ElectronProbe rdf:type owl:Class ;
               rdfs:subClassOf :Beam ;
               rdfs:comment "Häufig wird der Begriff Elektronensonde verwendet, um einen Punkt zu beschreiben, an dem der Strahl fokussiert ist. Der Begriff wird daher häufig im Zusammenhang mit fokussierten Strahlen verwendet."@de ,
                            "Often electron probe is used to describe a point where the beam is focused. It is commonly used in connection with focused beams."@en ;
               rdfs:isDefinedBy <https://w3id.org/pmd/mo> ;
               rdfs:label "Electron Probe"@en ,
                          "Elektronensonde"@de ;
               <http://www.w3.org/2004/02/skos/core#definition> "Der Teil des Strahls, der mit der Probe in Wechselwirkung tritt."@de ,
                                                                "The part of the beam which interacts with the sample."@en ;
               <https://w3id.org/pmd/co/definitionSource> <https://codebase.helmholtz.cloud/em_glossary/em_glossary/-/blob/main/terms/electron_probe.yaml> .


###  https://w3id.org/pmd/mo/ElectronProbeMicroAnalyzer
:ElectronProbeMicroAnalyzer rdf:type owl:Class ;
                            rdfs:subClassOf :ElectronMicroprobe ;
                            rdfs:isDefinedBy <https://w3id.org/pmd/mo> ;
                            rdfs:label "Electron Probe Micro Analyzer"@en ,
                                       "Elektronensonden-Mikro-Analysator"@de ;
                            <http://www.w3.org/2004/02/skos/core#definition> "An instrument used for elemental analysis of solid materials by bombarding them with a focused electron beam."@en ,
                                                                             "Ein Instrument zur Elementaranalyse fester Materialien durch Beschuss mit einem fokussierten Elektronenstrahl."@de ;
                            <https://w3id.org/pmd/co/definitionSource> "ChatGPT 3.5"@en .


###  https://w3id.org/pmd/mo/ElectronTomograph
:ElectronTomograph rdf:type owl:Class ;
                   rdfs:subClassOf :TransmissionElectronMicroscope ;
                   rdfs:isDefinedBy <https://w3id.org/pmd/mo> ;
                   rdfs:label "Electron Tomograph"@en ,
                              "Elektronentomograph"@de ;
                   <http://www.w3.org/2004/02/skos/core#definition> "An instrument used for tomographic imaging using electrons."@en ,
                                                                    "Ein Instrument für die tomografische Bildgebung mit Elektronen."@de ;
                   <https://w3id.org/pmd/co/definitionSource> "ChatGPT 3.5"@en ;
                   :abbreviation "ET"@en .


###  https://w3id.org/pmd/mo/ElectronTomography
:ElectronTomography rdf:type owl:Class ;
                    rdfs:subClassOf :TransmissionElectronMicroscopy ;
                    rdfs:isDefinedBy <https://w3id.org/pmd/mo> ;
                    rdfs:label "Electron Tomography"@en ,
                               "Elektronentomographie"@de ;
                    <http://www.w3.org/2004/02/skos/core#definition> "Electron Tomography is a technique that involves collecting a series of transmission electron microscopy (TEM) images from different angles to reconstruct a three-dimensional image of a sample."@en ;
                    <https://w3id.org/pmd/co/definitionSource> "ChatGPT 3.5"@en ;
                    :abbreviation "ET"@en .


###  https://w3id.org/pmd/mo/EmissionCurrent
:EmissionCurrent rdf:type owl:Class ;
                 rdfs:subClassOf :Current ;
                 rdfs:comment "Der Emissionsstrom ist eine geräte- und komponentenabhängige numerische Eigenschaft, die im Laufe der Zeit überwacht werden kann, um z. B. die Lebensdauer und den Verschleiß einer Quelle zu bewerten. Er ist nicht hersteller- oder geräteübergreifend vergleichbar."@de ,
                              "Emission current is a device- and component-dependent numerical property that can be monitored over time to evaluate e.g. service life and wear of a source. It is not cross-vendor or cross-device comparable."@en ;
                 rdfs:isDefinedBy <https://w3id.org/pmd/mo> ;
                 rdfs:label "Emission Current"@en ,
                            "Emissionsstrom"@de ;
                 <http://www.w3.org/2004/02/skos/core#definition> "Electrical current which is released from the source."@en ,
                                                                  "Elektrischer Strom, der von der Quelle abgegeben wird."@de ;
                 <https://w3id.org/pmd/co/definitionSource> <https://codebase.helmholtz.cloud/em_glossary/em_glossary/-/blob/main/terms/emission_current.yaml> .


###  https://w3id.org/pmd/mo/Energy
:Energy rdf:type owl:Class ;
        rdfs:subClassOf <https://w3id.org/pmd/co/ValueObject> ;
        rdfs:comment "Die Energie wird üblicherweise in Joule (J) oder Elektronenvolt (eV) gemessen."@de ,
                     "The energy is usually measured in joules (J) or electron volts (eV)."@en ;
        rdfs:isDefinedBy <https://w3id.org/pmd/mo> ;
        rdfs:label "Energie"@de ,
                   "Energy"@en ;
        <http://www.w3.org/2004/02/skos/core#definition> "Die Fähigkeit eines physischen Systems, Arbeit zu verrichten."@de ,
                                                         "The capacity of a physical system to perform work."@en ;
        <https://w3id.org/pmd/co/definitionSource> "ChatGPT 3.5"@en .


###  https://w3id.org/pmd/mo/EnergyDispersiveXRaySpectroscopy
:EnergyDispersiveXRaySpectroscopy rdf:type owl:Class ;
                                  rdfs:subClassOf :XRayMicroanalysis ;
                                  rdfs:isDefinedBy <https://w3id.org/pmd/mo> ;
                                  rdfs:label "Energy Dispersive X-ray Spectroscopy"@en ;
                                  <http://www.w3.org/2004/02/skos/core#altLabel> "energiedispersive Röntgenmikroanalyse"@de ;
                                  <http://www.w3.org/2004/02/skos/core#definition> "Energy Dispersive X-ray Spectroscopy is a technique used to analyze the elemental composition of a sample by detecting the X-rays emitted when the sample is bombarded with electrons in an electron microscope or other instrument. EDS provides information about the elements present in the sample and their relative concentrations."@en ;
                                  <http://www.w3.org/2004/02/skos/core#prefLabel> "energiedispersive Röntgenanalyse"@de ;
                                  <https://w3id.org/pmd/co/definitionSource> "ChatGPT 3.5"@en ;
                                  :abbreviation "EDS"@en ,
                                                "EDX"@en ,
                                                "XEDS"@en .


###  https://w3id.org/pmd/mo/EnergyFilteredTransmissionElectronMicroscope
:EnergyFilteredTransmissionElectronMicroscope rdf:type owl:Class ;
                                              rdfs:subClassOf :TransmissionElectronMicroscope ;
                                              rdfs:isDefinedBy <https://w3id.org/pmd/mo> ;
                                              rdfs:label "Energiegefiltertes Transmissionselektronenmikroskop"@de ,
                                                         "Energy-filtered Transmission Electron Microscope"@en ;
                                              <http://www.w3.org/2004/02/skos/core#definition> "A transmission electron microscope equipped with an energy filter to select electrons of specific energy levels."@en ,
                                                                                               "Ein Transmissionselektronenmikroskop, das mit einem Energiefilter ausgestattet ist, um Elektronen bestimmter Energieniveaus zu selektieren."@de ;
                                              <https://w3id.org/pmd/co/definitionSource> "ChatGPT 3.5"@en .


###  https://w3id.org/pmd/mo/EnergyLoss
:EnergyLoss rdf:type owl:Class ;
            rdfs:subClassOf :Energy ;
            rdfs:isDefinedBy <https://w3id.org/pmd/mo> ;
            rdfs:label "Energieverlust"@de ,
                       "Energy Loss"@en ;
            <http://www.w3.org/2004/02/skos/core#definition> "Der Energieverlust, den ein Teilchen beim Durchgang durch ein Medium erfährt."@de ,
                                                             "The loss of energy experienced by a particle as it passes through a medium."@en ;
            <https://w3id.org/pmd/co/definitionSource> "ChatGPT 3.5"@en .


###  https://w3id.org/pmd/mo/EnergyResolution
:EnergyResolution rdf:type owl:Class ;
                  rdfs:subClassOf :Resolution ;
                  rdfs:isDefinedBy <https://w3id.org/pmd/mo> ;
                  rdfs:label "Energieauflösung"@de ,
                             "Energy Resolution"@en ;
                  <http://www.w3.org/2004/02/skos/core#definition> "Die Fähigkeit eines Detektors, zwischen verschiedenen Energieniveaus der einfallenden Strahlung zu unterscheiden."@de ,
                                                                   "The ability of a detector to distinguish between different energy levels of incident radiation."@en ;
                  <https://w3id.org/pmd/co/definitionSource> "ChatGPT 3.5"@en .


###  https://w3id.org/pmd/mo/EnvironmentalScanningElectronMicroscope
:EnvironmentalScanningElectronMicroscope rdf:type owl:Class ;
                                         rdfs:subClassOf :ScanningElectronMicroscope ;
                                         rdfs:isDefinedBy <https://w3id.org/pmd/mo> ;
                                         rdfs:label "Environmental Scanning Electron Microscope"@en ,
                                                    "Umwelt-Rasterelektronenmikroskop"@de ;
                                         <http://www.w3.org/2004/02/skos/core#definition> "A type of electron microscope that can image non-conductive samples in their natural state."@en ,
                                                                                          "Eine Art Elektronenmikroskop, das nicht leitende Proben in ihrem natürlichen Zustand abbilden kann."@de ;
                                         <https://w3id.org/pmd/co/definitionSource> "ChatGPT 3.5"@en ;
                                         :abbreviation "ESEM"@en .


###  https://w3id.org/pmd/mo/EnvironmentalScanningElectronMicroscopy
:EnvironmentalScanningElectronMicroscopy rdf:type owl:Class ;
                                         rdfs:subClassOf :ScanningElectronMicroscopy ;
                                         rdfs:isDefinedBy <https://w3id.org/pmd/mo> ;
                                         rdfs:label "Environmental Scanning Electron Microscopy"@en ,
                                                    "Umgebungs-Rasterelektronenmikroskopie"@de ;
                                         <http://www.w3.org/2004/02/skos/core#definition> "Environmental Scanning Electron Microscopy is a technique that allows imaging of samples in a gaseous environment. It is particularly useful for observing hydrated or non-conductive samples without the need for extensive sample preparation."@en ;
                                         <https://w3id.org/pmd/co/definitionSource> "ChatGPT 3.5"@en ;
                                         :abbreviation "ESEM"@en .


###  https://w3id.org/pmd/mo/EnvironmentalTransmissionElectronMicroscopy
:EnvironmentalTransmissionElectronMicroscopy rdf:type owl:Class ;
                                             rdfs:subClassOf :TransmissionElectronMicroscopy ;
                                             rdfs:isDefinedBy <https://w3id.org/pmd/mo> ;
                                             rdfs:label "Environmental Transmission Electron Microscopy"@en ,
                                                        "Umgebungs-Transmissionselektronenmikroskopie"@de ;
                                             <http://www.w3.org/2004/02/skos/core#definition> "Environmental Transmission Electron Microscopy allows imaging and analysis of materials in controlled gaseous environments, simulating real-world conditions."@en ;
                                             <https://w3id.org/pmd/co/definitionSource> "ChatGPT 3.5"@en ;
                                             :abbreviation "ETEM"@en .


###  https://w3id.org/pmd/mo/ExtractionVoltage
:ExtractionVoltage rdf:type owl:Class ;
                   rdfs:subClassOf :Voltage ;
                   rdfs:comment "Die Extraktionsspannung wird bei Schottky- und Kaltfeldemissions-Elektronenquellen angelegt, nicht jedoch bei thermionischen Emittern. Sie soll dazu beitragen, dass Elektronen aus dem Inneren des Quellenmaterials emittiert werden, um die Arbeitsfunktion zu überwinden und emittiert zu werden. Gallium-Flüssigmetall-Ionenquellen verwenden ebenfalls eine Extraktionsspannung, um Ionen zu erzeugen. Höhere Extraktionsspannungen führen zu höheren Strahlströmen."@de ,
                                "Extraction voltage is applied to Schottky and Cold Field Emission electron sources, but not to thermionic emitters. It's purpose is to help emit electrons from inside the  source material to overcome the work function and be emitted. Gallium liquid metal  ion sources also use an extraction voltage to produce ions. Higher extraction voltages  will lead to higher beam currents."@en ;
                   rdfs:isDefinedBy <https://w3id.org/pmd/mo> ;
                   rdfs:label "Extraction Voltage"@en ,
                              "Extraktionsspannung"@de ;
                   <http://www.w3.org/2004/02/skos/core#definition> "Spannung, mit der ein elektrisches Feld erzeugt wird, das Partikel von der Quelle anzieht."@de ,
                                                                    "Voltage which is utilised to create an electric field that draws particles from the source."@en ;
                   <https://w3id.org/pmd/co/definitionSource> <https://codebase.helmholtz.cloud/em_glossary/em_glossary/-/blob/main/terms/extraction_voltage.yaml> .


###  https://w3id.org/pmd/mo/FieldEmissionGun
:FieldEmissionGun rdf:type owl:Class ;
                  rdfs:subClassOf :Gun ;
                  rdfs:isDefinedBy <https://w3id.org/pmd/mo> ;
                  rdfs:label "Feldemissionskanone"@de ,
                             "Field Emission Gun"@en ;
                  <http://www.w3.org/2004/02/skos/core#definition> "A Field Emission Gun is an electron gun used in electron microscopes to produce an electron beam with extremely high brightness and coherence. It relies on the phenomenon of field emission, where electrons are emitted from a sharp emitter tip under the influence of a strong electric field. FEGs are capable of producing highly focused electron beams, leading to enhanced imaging resolution and analytical capabilities."@en ;
                  <https://w3id.org/pmd/co/definitionSource> "ChatGPT 3.5"@en ;
                  :abbreviation "FEG"@en .


###  https://w3id.org/pmd/mo/FieldEmissionScanningElectronMicroscopy
:FieldEmissionScanningElectronMicroscopy rdf:type owl:Class ;
                                         rdfs:subClassOf :ScanningElectronMicroscopy ;
                                         rdfs:isDefinedBy <https://w3id.org/pmd/mo> ;
                                         rdfs:label "Feldemissions-Rasterelektronenmikroskopie"@de ,
                                                    "Field Emission Scanning Electron Microscopy"@en ;
                                         <http://www.w3.org/2004/02/skos/core#definition> "Field Emission Scanning Electron Microscopy is an advanced form of SEM that uses a field emitter to produce a highly focused electron beam, enabling high-resolution imaging and surface analysis."@en ;
                                         <https://w3id.org/pmd/co/definitionSource> "ChatGPT 3.5"@en ;
                                         :abbreviation "FESEM"@en .


###  https://w3id.org/pmd/mo/FieldIonMicroscope
:FieldIonMicroscope rdf:type owl:Class ;
                    rdfs:subClassOf :IonMicroscope ;
                    rdfs:isDefinedBy <https://w3id.org/pmd/mo> ;
                    rdfs:label "Feldionenmikroskop"@de ,
                               "Field Ion Microscope"@en ;
                    <http://www.w3.org/2004/02/skos/core#definition> "A type of microscope that uses the phenomenon of field ionization to image surfaces with atomic resolution."@en ,
                                                                     "Ein Mikroskoptyp, der das Phänomen der Feldionisation nutzt, um Oberflächen mit atomarer Auflösung abzubilden."@de ;
                    <https://w3id.org/pmd/co/definitionSource> "ChatGPT 3.5"@en ;
                    :abbreviation "FIM"@en .


###  https://w3id.org/pmd/mo/FieldIonMicroscopy
:FieldIonMicroscopy rdf:type owl:Class ;
                    rdfs:subClassOf :IonMicroscopy ;
                    rdfs:isDefinedBy <https://w3id.org/pmd/mo> ;
                    rdfs:label "Feldionenmikroskopie"@de ,
                               "Field Ion Microscopy"@en ;
                    <http://www.w3.org/2004/02/skos/core#definition> "Field Ion Microscopy is a specialized microscopy technique that uses a strong electric field to ionize atoms on the surface of a metal sample. These ionized atoms are then repelled from the surface and can be detected to create an image of the sample's surface topography at atomic resolution. FIM is especially powerful for imaging the arrangement of atoms on metallic surfaces."@en ;
                    <https://w3id.org/pmd/co/definitionSource> "ChatGPT 3.5"@en ;
                    :abbreviation "FIM"@en .


###  https://w3id.org/pmd/mo/FilamentCurrent
:FilamentCurrent rdf:type owl:Class ;
                 rdfs:subClassOf :Current ;
                 rdfs:comment "Dieser wird in der Regel zum Heizen einer Quelle verwendet und liefert den Emissionsstrom. Höhere Glühfadenströme führen zu höheren Strahlströmen."@de ,
                              "This is typically used for heating a source and supplies the emission  current. Higher filament currents will result in higher beam currents."@en ;
                 rdfs:isDefinedBy <https://w3id.org/pmd/mo> ;
                 rdfs:label "Filament Current"@en ,
                            "Glühfadenstrom"@de ;
                 <http://www.w3.org/2004/02/skos/core#definition> "Electrical current which flows through the source."@en ,
                                                                  "Elektrischer Strom, der durch die Quelle fließt."@de ;
                 <https://w3id.org/pmd/co/definitionSource> <https://codebase.helmholtz.cloud/em_glossary/em_glossary/-/blob/main/terms/filament_current.yaml> .


###  https://w3id.org/pmd/mo/FluorescenceMicroscopy
:FluorescenceMicroscopy rdf:type owl:Class ;
                        rdfs:subClassOf :LightMicroscopy ;
                        rdfs:isDefinedBy <https://w3id.org/pmd/mo> ;
                        rdfs:label "Fluorescence Microscopy"@en ,
                                   "Fluoreszenzmikroskopie"@de ;
                        <http://www.w3.org/2004/02/skos/core#definition> "Fluorescence Microscopy is an optical imaging technique used to visualize biological structures and molecules that fluoresce when illuminated with specific wavelengths of light. Fluorescent molecules absorb light energy and then emit light of a longer wavelength, allowing the visualization of specific molecules or cellular components. Fluorescence microscopy is widely used in cell biology, molecular biology, and medical research."@en ;
                        <https://w3id.org/pmd/co/definitionSource> "ChatGPT 3.5"@en .


###  https://w3id.org/pmd/mo/FlybackTime
:FlybackTime rdf:type owl:Class ;
             rdfs:subClassOf <https://w3id.org/pmd/co/Duration> ;
             rdfs:comment "Die Rücklaufzeit wird in der Regel mit rechteckigen Abtastmustern in Verbindung gebracht und in den Metadaten der Hersteller oft als solche beschrieben. Ein typisches geometrisches Primitiv für rechteckige Abtastungen sind Linien. Die Rücklaufzeit kann als ein spezielles Beispiel für die Wartezeit betrachtet werden, allerdings können einige Geräte auch während der Rücklaufzeit Daten erfassen, weshalb sie in diesem Artefakt separat definiert wird."@de ,
                          "Flyback time is commonly associated with rectangular scan patterns and often described in metadata from vendors as such. A typical geometrical primitive for rectangular scans are lines. Flyback time may be considered a specific  instance of wait time, however some instruments might still be able to acquire  data during flyback time which is why it is defined separately in this artefact."@en ;
             rdfs:isDefinedBy <https://w3id.org/pmd/mo> ;
             rdfs:label "Flyback Time"@en ,
                        "Rücklaufzeit"@de ;
             <http://www.w3.org/2004/02/skos/core#definition> "Time period during which the beam moves from the final position of one scan line to the starting position of the subsequent scan line."@en ,
                                                              "Zeitspanne, in der sich der Strahl von der Endposition einer Scanlinie zur Startposition der nächsten Scanlinie bewegt."@de ;
             <https://w3id.org/pmd/co/definitionSource> <https://codebase.helmholtz.cloud/em_glossary/em_glossary/-/blob/main/terms/flyback_time.yaml> .


###  https://w3id.org/pmd/mo/FocalLength
:FocalLength rdf:type owl:Class ;
             rdfs:subClassOf <https://w3id.org/pmd/co/Length> ;
             rdfs:comment "A beam consisting of parallel rays converges into one point for positive focal lengths. The focal length is an inherent property of a lens."@en ,
                          "Ein aus parallelen Strahlen bestehender Strahl konvergiert bei positiven Brennweiten in einem Punkt. Die Brennweite ist eine inhärente Eigenschaft einer Linse."@de ;
             rdfs:isDefinedBy <https://w3id.org/pmd/mo> ;
             rdfs:label "Brennweite"@de ,
                        "Focal Length"@en ;
             <http://www.w3.org/2004/02/skos/core#definition> "Abstand zwischen der Hauptebene des Objektivs und dem Brennpunkt entlang der optischen Achse."@de ,
                                                              "Distance which lies between the principal plane of the lens and the focal point along the optical axis."@en ;
             <https://w3id.org/pmd/co/definitionSource> <https://codebase.helmholtz.cloud/em_glossary/em_glossary/-/blob/main/terms/focal_length.yaml> .


###  https://w3id.org/pmd/mo/FocalPlane
:FocalPlane rdf:type owl:Class ;
            rdfs:subClassOf <https://w3id.org/pmd/co/Area> ;
            rdfs:comment "Die Ebene befindet sich in der Regel auf dem Probekörper."@de ,
                         "The plane is typically on the specimen."@en ;
            rdfs:isDefinedBy <https://w3id.org/pmd/mo> ;
            rdfs:label "Brennebene"@de ,
                       "Focal Plane"@en ;
            <http://www.w3.org/2004/02/skos/core#altLabel> "Front Focal Plane"@en ,
                                                           "Vordere Brennebene"@de ;
            <http://www.w3.org/2004/02/skos/core#definition> "Ebene, die senkrecht zur optischen Achse liegt und den Brennpunkt einschließt."@de ,
                                                             "Plane which is perpendicular to the optical axis and includes the focal point."@en ;
            <https://w3id.org/pmd/co/definitionSource> <https://codebase.helmholtz.cloud/em_glossary/em_glossary/-/blob/main/terms/focal_plane.yaml> .


###  https://w3id.org/pmd/mo/FocalPoint
:FocalPoint rdf:type owl:Class ;
            rdfs:subClassOf <https://w3id.org/pmd/co/DigitalEntity> ;
            rdfs:comment "Die hier gegebene Definition gilt für elektromagnetische Linsen und ist eine allgemeinere Definition im Vergleich zu den in der klassischen Optik üblichen Definitionen. Der Brennpunkt ist eine inhärente Eigenschaft einer Linse. Die Definition gilt nur, wenn sich die (virtuelle) Quelle \"im Unendlichen\" befindet, d. h. sehr weit entfernt im Vergleich zur Brennweite des Objektivs. Dies gilt für ein ideales Objektiv; in der Realität kann es zu Abbildungsfehlern kommen, die das Strahlprofil im Brennpunkt beeinflussen."@de ,
                         "The here given definition applies to electromagnetic lenses and is a more general definition compared to those typically given in classical optics. The focal point is an inherent property of a lens. Definition only holds if the (virtual) source is \"at infinity\", meaning very far away as compared to the focal length of the objective lens. This is for an ideal lens, in the reality there might be aberrations affecting the beam profile at the focal point."@en ;
            rdfs:isDefinedBy <https://w3id.org/pmd/mo> ;
            rdfs:label "Brennpunkt"@de ,
                       "Focal Point"@en ;
            <http://www.w3.org/2004/02/skos/core#definition> "Point at which the optical axis is crossed by backwards extrapolated path of a ray that (1) is tending towards infinity, (2) was parallel to the optical axis in the incident beam, and (3) that was deflected by an electron lens."@en ,
                                                             "Punkt, an dem die optische Achse von der rückwärts extrapolierten Bahn eines Strahls gekreuzt wird, der (1) ins Unendliche tendiert, (2) im einfallenden Strahl parallel zur optischen Achse verlief und (3) durch eine Elektronenlinse abgelenkt wurde."@de ;
            <https://w3id.org/pmd/co/definitionSource> <https://codebase.helmholtz.cloud/em_glossary/em_glossary/-/blob/main/terms/focal_point.yaml> ,
                                                       <https://www.iso.org/obp/ui/#iso:std:iso:15932:ed-1:v1:en_2.1.4> ,
                                                       <https://www.iso.org/obp/ui/#iso:std:iso:22493:ed-2:v1:en_3.1.4> .


###  https://w3id.org/pmd/mo/FocusedBeam
:FocusedBeam rdf:type owl:Class ;
             rdfs:subClassOf :Beam ;
             rdfs:comment "Die Begriffe fokussierter Strahl und konvergenter Strahl werden umgangssprachlich oft fast gleichbedeutend verwendet. Hier werden diese Begriffe unterschieden, indem darauf hinweisen wird, dass fokussierte Strahlen mit der Absicht verwendet werden, den Strahl auf den physikalisch kleinstmöglichen Bereich zu richten."@de ,
                          "The terms focused beam and convergent beam are colloquially often used almost interchangeably. Here, these terms are differentiated by pointing to focused beams being used with the intention to direct the beam to the physically smallest possible area."@en ;
             rdfs:isDefinedBy <https://w3id.org/pmd/mo> ;
             rdfs:label "Focused Beam"@en ,
                        "Fokussierter Strahl"@de ;
             <http://www.w3.org/2004/02/skos/core#altLabel> "Gebündelter Strahl"@de ;
             <http://www.w3.org/2004/02/skos/core#definition> "A convergent beam which originates from a coherent beam and whose cross section is decreased to the physically smallest possible disc of least confusion."@en ,
                                                              "Ein konvergierender Strahl, der von einem kohärenten Strahl ausgeht und dessen Querschnitt auf die physikalisch kleinstmögliche Scheibe der geringsten Konfusion reduziert ist."@de ;
             <https://w3id.org/pmd/co/definitionSource> <https://codebase.helmholtz.cloud/em_glossary/em_glossary/-/blob/main/terms/focused_beam.yaml> .


###  https://w3id.org/pmd/mo/FocusedIonBeam-ScanningElectronMicroscope
:FocusedIonBeam-ScanningElectronMicroscope rdf:type owl:Class ;
                                           rdfs:subClassOf :IonMicroscope ;
                                           rdfs:isDefinedBy <https://w3id.org/pmd/mo> ;
                                           rdfs:label "Focus(ed) Ion Beam - Scanning Electron Microscope"@en ,
                                                      "Fokussierter Ionenstrahl - Rasterelektronenmikroskop"@de ;
                                           <http://www.w3.org/2004/02/skos/core#definition> "A dual-beam microscope that combines a focused ion beam with a scanning electron microscope."@en ,
                                                                                            "Ein Zweistrahlmikroskop, das einen fokussierten Ionenstrahl mit einem Rasterelektronenmikroskop kombiniert."@de ;
                                           <https://w3id.org/pmd/co/definitionSource> "ChatGPT 3.5"@en ;
                                           :abbreviation "FIB-SEM"@en .


###  https://w3id.org/pmd/mo/FocusedIonBeamScanningElectronMicroscopy
:FocusedIonBeamScanningElectronMicroscopy rdf:type owl:Class ;
                                          rdfs:subClassOf :IonMicroscopy ;
                                          rdfs:isDefinedBy <https://w3id.org/pmd/mo> ;
                                          rdfs:label "Focused Ion Beam Scanning Electron Microscopy"@en ,
                                                     "Fokussierte Ionenstrahl-Rasterelektronenmikroskopie"@de ;
                                          <http://www.w3.org/2004/02/skos/core#definition> "Focused Ion Beam Scanning Electron Microscopy is a combination of two techniques: focused ion beam (FIB) and scanning electron microscopy (SEM). FIB-SEM systems use a focused ion beam to both image and modify a sample's surface. The ion beam can be used for milling, cutting, and deposition processes, making FIB-SEM a versatile tool for materials analysis, sample preparation, and three-dimensional imaging."@en ;
                                          <https://w3id.org/pmd/co/definitionSource> "ChatGPT 3.5"@en ;
                                          :abbreviation "FIB-SEM"@en .


###  https://w3id.org/pmd/mo/FourierTransformInfraredSpectroscopy
:FourierTransformInfraredSpectroscopy rdf:type owl:Class ;
                                      rdfs:subClassOf :Spectroscopy ;
                                      rdfs:isDefinedBy <https://w3id.org/pmd/mo> ;
                                      rdfs:label "Fourier Transform Infrared Spectroscopy"@en ,
                                                 "Fourier-Transformations-Infrarotspektroskopie"@de ;
                                      <http://www.w3.org/2004/02/skos/core#definition> """Fourier Transform Infrared Spectroscopy (FTIR) is a powerful analytical technique used in various scientific disciplines to study the molecular composition and properties of materials. It is based on the interaction between infrared radiation and a sample, providing information about the vibrational modes of molecules.
In FTIR spectroscopy, an infrared beam is directed through a sample, and the interaction between the radiation and the sample's molecules leads to absorption of specific infrared frequencies. Each type of molecular bond and functional group in the sample absorbs infrared radiation at characteristic frequencies, which correspond to the energies of molecular vibrations. The resulting absorption spectrum represents a fingerprint of the sample's molecular structure.
The Fourier transform technique is used to convert the raw data obtained from the absorption measurements into a Fourier-transformed spectrum. This transformation improves the signal-to-noise ratio and enhances the accuracy of spectral analysis.
FTIR is extensively used in a wide range of fields, including chemistry, biology, materials science, pharmaceuticals, and environmental science. It is employed for qualitative and quantitative analysis, identification of compounds, monitoring chemical reactions, and studying molecular interactions. FTIR spectroscopy provides valuable insights into molecular bonding, functional groups, and the chemical composition of substances, making it an indispensable tool in modern analytical science."""@en ;
                                      <https://w3id.org/pmd/co/definitionSource> "ChatGPT 3.5"@en ;
                                      :abbreviation "FTIR"@en .


###  https://w3id.org/pmd/mo/FrameFlybackTime
:FrameFlybackTime rdf:type owl:Class ;
                  rdfs:subClassOf :FlybackTime ;
                  rdfs:comment "Die Rahmen-Rücklaufzeit kann als ein spezieller Fall von Wartezeit betrachtet werden, allerdings können einige Geräte auch während der Rahmen-Rücklaufzeit Daten erfassen, weshalb sie in diesem Artefakt separat definiert wird."@de ,
                               "Frame flyback time may be considered a specific instance of wait time, however some instruments might still be able to acquire data during frame flyback time which is why it is defined separately in this artefact."@en ;
                  rdfs:isDefinedBy <https://w3id.org/pmd/mo> ;
                  rdfs:label "Frame Flyback Time"@en ,
                             "Rahmen-Rücklaufzeit"@de ;
                  <http://www.w3.org/2004/02/skos/core#definition> "Time period during which the beam moves from the final position of one frame to the starting position of the subsequent frame."@en ,
                                                                   "Zeitspanne, in der sich der Strahl von der Endposition eines Bildes zur Startposition des nächsten Bildes bewegt."@de ;
                  <https://w3id.org/pmd/co/definitionSource> <https://codebase.helmholtz.cloud/em_glossary/em_glossary/-/blob/main/terms/frame_flyback_time.yaml> .


###  https://w3id.org/pmd/mo/FrameTime
:FrameTime rdf:type owl:Class ;
           rdfs:subClassOf <https://w3id.org/pmd/co/Duration> ;
           rdfs:comment "Die Rahmenscanzeit wird in der Regel durch eine gewichtete Summe aus folgenden Faktoren bestimmt: Verweilzeit, Bewegungszeiten und möglicherweise Wartezeit. Die Gewichtungsfaktoren werden durch das spezifische Scanmuster bestimmt."@de ,
                        "The frame time is typically determined by a weighted sum of: Dwell time, move times and potentially wait time. The weighting factors are determined by the specific scan pattern."@en ;
           rdfs:isDefinedBy <https://w3id.org/pmd/mo> ;
           rdfs:label "Frame Time"@en ,
                      "Rahmenscanzeit"@de ;
           <http://www.w3.org/2004/02/skos/core#definition> "Time period during which a frame is fully scanned."@en ,
                                                            "Zeitspanne, in der ein Bild (Rahmen, Frame) vollständig gescannt wird."@de ;
           <https://w3id.org/pmd/co/definitionSource> <https://codebase.helmholtz.cloud/em_glossary/em_glossary/-/blob/main/terms/frame_time.yaml> ,
                                                      <https://doi.org/10.1007/978-1-4939-6676-9> .


###  https://w3id.org/pmd/mo/GatanImageFilter
:GatanImageFilter rdf:type owl:Class ;
                  rdfs:subClassOf :ImageFilter ;
                  rdfs:isDefinedBy <https://w3id.org/pmd/mo> ;
                  rdfs:label "Gatan Abbildungsfilter"@de ,
                             "Gatan Image Filter"@en ;
                  <http://www.w3.org/2004/02/skos/core#definition> "A Gatan Image Filter refers to an image filter manufactured by Gatan, Inc., a company specializing in electron microscopy and related products. Gatan's image filters are designed for electron microscopes and electron energy loss spectroscopy (EELS) applications. These filters allow researchers to control and enhance the acquisition of electron energy loss spectra while obtaining high-resolution images of the sample under investigation."@en ;
                  <https://w3id.org/pmd/co/definitionSource> "ChatGPT 3.5"@en .


###  https://w3id.org/pmd/mo/Gun
:Gun rdf:type owl:Class ;
     rdfs:subClassOf <https://w3id.org/pmd/co/ProcessingNode> ;
     rdfs:isDefinedBy <https://w3id.org/pmd/mo> ;
     rdfs:label "Gun"@en ,
                "Kanone"@de ;
     <http://www.w3.org/2004/02/skos/core#definition> "In the context of electron microscopy and particle acceleration, a \"gun\" typically refers to an electron or particle source that generates and emits the particles. In electron microscopy, an electron gun is used to generate a beam of electrons for imaging or analysis. In particle accelerators, a particle gun generates and launches particles at high speeds for various experimental purposes."@en ;
     <https://w3id.org/pmd/co/definitionSource> "ChatGPT 3.5"@en .


###  https://w3id.org/pmd/mo/HeliumIonMicroscope
:HeliumIonMicroscope rdf:type owl:Class ;
                     rdfs:subClassOf :FocusedIonBeam-ScanningElectronMicroscope ;
                     rdfs:isDefinedBy <https://w3id.org/pmd/mo> ;
                     rdfs:label "Helium Ion Microscope"@en ,
                                "Helium-Ionen-Mikroskop"@de ;
                     <http://www.w3.org/2004/02/skos/core#definition> "A type of microscope that uses helium ions to image samples with high resolution."@en ,
                                                                      "Eine Art Mikroskop, das Helium-Ionen verwendet, um Proben mit hoher Auflösung abzubilden."@de ;
                     <https://w3id.org/pmd/co/definitionSource> "ChatGPT 3.5"@en ;
                     :abbreviation "HIM"@en .


###  https://w3id.org/pmd/mo/HeliumIonMicroscopy
:HeliumIonMicroscopy rdf:type owl:Class ;
                     rdfs:subClassOf :IonMicroscopy ;
                     rdfs:isDefinedBy <https://w3id.org/pmd/mo> ;
                     rdfs:label "Helium Ion Microscopy"@en ,
                                "Helium-Ionen-Mikroskopie"@de ;
                     <http://www.w3.org/2004/02/skos/core#definition> "Helium Ion Microscopy is a microscopy technique that uses a beam of helium ions instead of electrons to interact with a sample's surface. The smaller mass of helium ions compared to electrons allows for higher resolution imaging and reduced sample damage. HIM provides high-resolution images and is often used for imaging delicate or sensitive samples."@en ;
                     <https://w3id.org/pmd/co/definitionSource> "ChatGPT 3.5"@en ;
                     :abbreviation "HIM"@en .


###  https://w3id.org/pmd/mo/HighAngleAnnularDarkFieldScanningTransmissionElectronMicroscope
:HighAngleAnnularDarkFieldScanningTransmissionElectronMicroscope rdf:type owl:Class ;
                                                                 rdfs:subClassOf :ScanningTransmissionElectronMicroscope ;
                                                                 rdfs:isDefinedBy <https://w3id.org/pmd/mo> ;
                                                                 rdfs:label "High-angle Annular Dark-field Scanning Transmission Electron Microscope"@en ,
                                                                            "Hochwinkel-Dunkelfeld-Rastertransmissionselektronenmikroskop mit annularem Winkel"@de ;
                                                                 <http://www.w3.org/2004/02/skos/core#definition> "A type of scanning transmission electron microscope that detects scattered electrons at high angles."@en ,
                                                                                                                  "Eine Art Rastertransmissionselektronenmikroskop, das gestreute Elektronen in hohen Winkeln erkennt."@de ;
                                                                 <https://w3id.org/pmd/co/definitionSource> "ChatGPT 3.5"@en ;
                                                                 :abbreviation "HAADF-STEM"@en .


###  https://w3id.org/pmd/mo/HighResolutionTransmissionElectronMicroscope
:HighResolutionTransmissionElectronMicroscope rdf:type owl:Class ;
                                              rdfs:subClassOf :TransmissionElectronMicroscope ;
                                              rdfs:isDefinedBy <https://w3id.org/pmd/mo> ;
                                              rdfs:label "High Resolution Transmission Electron Microscope"@en ,
                                                         "Hochauflösendes Transmissionselektronenmikroskop"@de ;
                                              <http://www.w3.org/2004/02/skos/core#definition> "A transmission electron microscope capable of achieving high-resolution images."@en ,
                                                                                               "Ein Transmissionselektronenmikroskop, das hochauflösende Bilder liefert."@de ;
                                              <https://w3id.org/pmd/co/definitionSource> "ChatGPT 3.5"@en ;
                                              :abbreviation "HRTEM"@en .


###  https://w3id.org/pmd/mo/HighResolutionTransmissionElectronMicroscopy
:HighResolutionTransmissionElectronMicroscopy rdf:type owl:Class ;
                                              rdfs:subClassOf :TransmissionElectronMicroscopy ;
                                              rdfs:isDefinedBy <https://w3id.org/pmd/mo> ;
                                              rdfs:label "High Resolution Transmission Electron Microscopy"@en ,
                                                         "Hochauflösende Transmissionselektronenmikroskopie"@de ;
                                              <http://www.w3.org/2004/02/skos/core#definition> "High Resolution TEM is a technique that provides exceptionally high-resolution images of a sample's internal structure, revealing atomic-level details."@en ;
                                              <https://w3id.org/pmd/co/definitionSource> "ChatGPT 3.5"@en ;
                                              :abbreviation "HRTEM"@en .


###  https://w3id.org/pmd/mo/ImageFilter
:ImageFilter rdf:type owl:Class ;
             rdfs:subClassOf <https://w3id.org/pmd/co/ProcessingNode> ;
             rdfs:isDefinedBy <https://w3id.org/pmd/mo> ;
             rdfs:label "Abbildungsfilter"@de ,
                        "Image Filter"@en ;
             <http://www.w3.org/2004/02/skos/core#definition> "An image filter is a device or component used in imaging systems, such as microscopy or photography, to modify the appearance of an image by selectively altering certain characteristics. Filters can be used to adjust contrast, brightness, color balance, and other image properties. They are often used to enhance specific features or to correct for distortions caused by lighting conditions or optical imperfections."@en ;
             <https://w3id.org/pmd/co/definitionSource> "ChatGPT 3.5"@en .


###  https://w3id.org/pmd/mo/IncidentBeam
:IncidentBeam rdf:type owl:Class ;
              rdfs:subClassOf :Beam ;
              rdfs:comment "Ein einfallender Strahl kann nur in Gegenwart einer Probe auftreten. Einfallend in diesem Sinne ist ein Verb, das die Wirkung des Strahls beschreibt. Der Strahlengang eines einfallenden Strahls schneidet sich in der Regel mit der Probe."@de ,
                           "You can only have an incident beam in the presence of a specimen. Incident in this  sense is a verb used to describe the action of the beam. Typically the beam path of an incident beam intersects with the specimen."@en ;
              rdfs:isDefinedBy <https://w3id.org/pmd/mo> ;
              rdfs:label "Einfallender Strahl"@de ,
                         "Incident Beam"@en ;
              <http://www.w3.org/2004/02/skos/core#definition> "Primary beam before it interacts with the specimen."@en ,
                                                               "Primärstrahl, bevor er auf die Probe trifft."@de ;
              <http://www.w3.org/2004/02/skos/core#example> """- Beispiel für einen Begriff
- Beispiel für einen größeren Begriff
- Beispiel für eine Instanz"""@de ,
                                                            """- term example
- larger term example
- instance example"""@en ;
              <https://w3id.org/pmd/co/definitionSource> <https://codebase.helmholtz.cloud/em_glossary/em_glossary/-/blob/main/terms/incident_beam.yaml> ,
                                                         <https://www.iso.org/obp/ui/#iso:std:iso:15932:ed-1:v1:en> ,
                                                         <https://www.iso.org/obp/ui/#iso:std:iso:23833:ed-2:v1:en> .


###  https://w3id.org/pmd/mo/InelasticScattering
:InelasticScattering rdf:type owl:Class ;
                     rdfs:subClassOf :PhysicalProcess ;
                     rdfs:isDefinedBy <https://w3id.org/pmd/mo> ;
                     rdfs:label "Inelastic Scattering"@en ,
                                "Inelastische Streuung"@de ;
                     <http://www.w3.org/2004/02/skos/core#definition> "Inelastic scattering is a scattering process that involves the transfer of energy and momentum between the incident particle (e.g., photon, electron) and the target particle. During inelastic scattering, the energy of the scattered particle changes, and the interaction may result in various outcomes, such as excitation, emission, or other energy transfers that alter the internal state of the target particle."@en ;
                     <https://w3id.org/pmd/co/definitionSource> "ChatGPT 3.5"@en .


###  https://w3id.org/pmd/mo/InteractionVolume
:InteractionVolume rdf:type owl:Class ;
                   rdfs:subClassOf :Volume ;
                   rdfs:isDefinedBy <https://w3id.org/pmd/mo> ;
                   rdfs:label "Interaction Volume"@en ,
                              "Überlagerungsvolumen"@de ;
                   <http://www.w3.org/2004/02/skos/core#definition> "Der Bereich innerhalb einer Probe, in dem ein Teilchenstrahl mit dem Material in Wechselwirkung tritt."@de ,
                                                                    "The region within a sample where a particle beam interacts with the material."@en ;
                   <https://w3id.org/pmd/co/definitionSource> "ChatGPT 3.5"@en .


###  https://w3id.org/pmd/mo/IonBeam
:IonBeam rdf:type owl:Class ;
         rdfs:subClassOf :Beam ;
         rdfs:isDefinedBy <https://w3id.org/pmd/mo> ;
         rdfs:label "Ion Beam"@en ,
                    "Ionenstrahl"@de ;
         <http://www.w3.org/2004/02/skos/core#definition> "A beam which consists of ions."@en ,
                                                          "Ein Strahl, der aus Ionen besteht."@de ;
         <https://w3id.org/pmd/co/definitionSource> <https://codebase.helmholtz.cloud/em_glossary/em_glossary/-/blob/main/terms/ion_beam.yaml> .


###  https://w3id.org/pmd/mo/IonMicroscope
:IonMicroscope rdf:type owl:Class ;
               rdfs:subClassOf <https://w3id.org/pmd/co/Micropscope> ;
               rdfs:isDefinedBy <https://w3id.org/pmd/mo> ;
               rdfs:label "Ion Microscope"@en ,
                          "Ionenmikroskop"@de ;
               <http://www.w3.org/2004/02/skos/core#definition> "A microscope that uses ions to create images of samples."@en ,
                                                                "Ein Mikroskop, das mit Hilfe von Ionen Bilder von Proben erzeugt."@de ;
               <https://w3id.org/pmd/co/definitionSource> "ChatGPT 3.5"@en .


###  https://w3id.org/pmd/mo/IonMicroscopy
:IonMicroscopy rdf:type owl:Class ;
               rdfs:subClassOf <https://w3id.org/pmd/co/MicroscopyProcess> ;
               rdfs:isDefinedBy <https://w3id.org/pmd/mo> ;
               rdfs:label "Ion Microscopy"@en ,
                          "Ionenmikroskopie"@de ;
               <http://www.w3.org/2004/02/skos/core#definition> "Ion Microscopy refers to a group of microscopy techniques that use focused ion beams to image and analyze samples. These techniques utilize ions, such as protons or heavy ions, instead of electrons or photons to interact with the sample, providing valuable information about its composition and structure."@en ;
               <https://w3id.org/pmd/co/definitionSource> "ChatGPT 3.5"@en .


###  https://w3id.org/pmd/mo/LightMicroscope
:LightMicroscope rdf:type owl:Class ;
                 rdfs:subClassOf :OpticalMicroscope ;
                 rdfs:isDefinedBy <https://w3id.org/pmd/mo> ;
                 rdfs:label "Lichtmikroskop"@de ,
                            "Light Microscope"@en ;
                 <http://www.w3.org/2004/02/skos/core#definition> "An optical microscope that uses visible light to illuminate and magnify samples."@en ,
                                                                  "Ein optisches Mikroskop, das sichtbares Licht verwendet, um Proben zu beleuchten und zu vergrößern."@de ;
                 <https://w3id.org/pmd/co/definitionSource> "ChatGPT 3.5"@en .


###  https://w3id.org/pmd/mo/LightMicroscopy
:LightMicroscopy rdf:type owl:Class ;
                 rdfs:subClassOf <https://w3id.org/pmd/co/OpticalMicroscopy> ;
                 rdfs:isDefinedBy <https://w3id.org/pmd/mo> ;
                 rdfs:label "Lichtmikroskopie"@de ,
                            "Light Microscopy"@en ;
                 <http://www.w3.org/2004/02/skos/core#definition> "Die Verwendung von sichtbarem Licht zur Beobachtung und Untersuchung kleiner Objekte oder Strukturen."@de ,
                                                                  "The use of visible light to observe and study small objects or structures."@en ;
                 <https://w3id.org/pmd/co/definitionSource> "ChatGPT 3.5"@en .


###  https://w3id.org/pmd/mo/Magnification
:Magnification rdf:type owl:Class ;
               rdfs:subClassOf <https://w3id.org/pmd/co/ValueObject> ;
               rdfs:isDefinedBy <https://w3id.org/pmd/mo> ;
               rdfs:label "Magnification"@en ,
                          "Vergrößerung"@de ;
               <http://www.w3.org/2004/02/skos/core#definition> "Das Verhältnis zwischen der Größe eines von einem optischen System erzeugten Bildes und der Größe des Objekts."@de ,
                                                                "The ratio of the size of an image produced by an optical system to the size of the object."@en ;
               <https://w3id.org/pmd/co/definitionSource> "ChatGPT 3.5"@en .


###  https://w3id.org/pmd/mo/MechanicalPolishing
:MechanicalPolishing rdf:type owl:Class ;
                     rdfs:subClassOf <https://w3id.org/pmd/co/ManufacturingProcess> ;
                     rdfs:isDefinedBy <https://w3id.org/pmd/mo> ;
                     rdfs:label "Mechanical Polishing"@en ,
                                "Mechanisches Polieren"@de ;
                     <http://www.w3.org/2004/02/skos/core#definition> """Mechanical polishing is a material preparation technique used to enhance the surface quality and finish of a sample by removing thin layers of material through abrasion. It involves using abrasive materials, such as polishing cloths, diamond suspensions, or abrasive pastes, along with a polishing machine or device. The process typically includes several steps, each using progressively finer abrasives to achieve a smooth and mirror-like surface.

During mechanical polishing, the sample is pressed against the rotating polishing medium with controlled pressure. The abrasive particles embedded in the medium gradually remove surface irregularities, scratches, and imperfections, resulting in improved flatness, clarity, and reflectivity. The process can be adjusted to target specific levels of surface roughness and precision.

Mechanical polishing is commonly used in various scientific and industrial applications, such as metallography, materials science, electronics, and optics. It is an essential step before further analyses like microscopy, spectroscopy, or surface profiling, as it provides a pristine surface for accurate characterization and observation of material properties."""@en ;
                     <https://w3id.org/pmd/co/definitionSource> "ChatGPT 3.5"@en .


###  https://w3id.org/pmd/mo/MonochromaticBeam
:MonochromaticBeam rdf:type owl:Class ;
                   rdfs:subClassOf :Beam ;
                   rdfs:comment "According to the wave particle dualism the here given definition translates also to a beam which consists of waves having the same wavelength. Note that in practice, absolute monochromaticity cannot be achieved and consequently a small energy spread always persists."@en ,
                                "Gemäß dem Welle-Teilchen-Dualismus lässt sich die hier gegebene Definition auch auf einen Strahl übertragen, der aus Wellen mit der gleichen Wellenlänge besteht. Es ist zu beachten, dass in der Praxis eine absolute Monochromatizität nicht erreicht werden kann und daher immer eine kleine Energiespanne bestehen bleibt."@de ;
                   rdfs:isDefinedBy <https://w3id.org/pmd/mo> ;
                   rdfs:label "Monochromatic Beam"@en ,
                              "Monochromatischer Strahl"@de ;
                   <http://www.w3.org/2004/02/skos/core#definition> "A beam which consists of particles of the same energy."@en ,
                                                                    "Ein Strahl, der aus Teilchen der gleichen Energie besteht."@de ;
                   <https://w3id.org/pmd/co/definitionSource> <https://codebase.helmholtz.cloud/em_glossary/em_glossary/-/blob/main/terms/monochromatic_beam.yaml> .


###  https://w3id.org/pmd/mo/Monochromator
:Monochromator rdf:type owl:Class ;
               rdfs:subClassOf <https://w3id.org/pmd/co/ProcessingNode> ;
               rdfs:isDefinedBy <https://w3id.org/pmd/mo> ;
               rdfs:label "Monochromator"@de ,
                          "Monochromator"@en ;
               <http://www.w3.org/2004/02/skos/core#definition> "An optical device that transmits a narrow range of wavelengths of light."@en ,
                                                                "Ein optisches Gerät, das einen engen Wellenlängenbereich von Licht überträgt."@de ;
               <https://w3id.org/pmd/co/definitionSource> "ChatGPT 3.5"@en .


###  https://w3id.org/pmd/mo/OpticalMicroscope
:OpticalMicroscope rdf:type owl:Class ;
                   rdfs:subClassOf <https://w3id.org/pmd/co/Micropscope> ;
                   rdfs:isDefinedBy <https://w3id.org/pmd/mo> ;
                   rdfs:label "Optical Microscope"@en ,
                              "Optisches Mikroskop"@de ;
                   <http://www.w3.org/2004/02/skos/core#definition> "A microscope that uses visible light and lenses to magnify specimens."@en ,
                                                                    "Ein Mikroskop, das sichtbares Licht und Linsen zur Vergrößerung von Proben verwendet."@de ;
                   <https://w3id.org/pmd/co/definitionSource> "ChatGPT 3.5"@en .


###  https://w3id.org/pmd/mo/OrientationImagingMicroscopy
:OrientationImagingMicroscopy rdf:type owl:Class ;
                              rdfs:subClassOf :ScanningElectronMicroscopy ;
                              rdfs:isDefinedBy <https://w3id.org/pmd/mo> ;
                              rdfs:label "Bildgebende Orientierungsmikroskopie"@de ,
                                         "Orientation Imaging Microscopy"@en ;
                              <http://www.w3.org/2004/02/skos/core#definition> "Orientation Imaging Microscopy is a microscopy technique used to map the crystallographic orientations of grains within a material. It is commonly applied in SEM to study the microstructural properties of polycrystalline materials."@en ;
                              <https://w3id.org/pmd/co/definitionSource> "ChatGPT 3.5"@en ;
                              :abbreviation "OIM"@en .


###  https://w3id.org/pmd/mo/PhysicalProcess
:PhysicalProcess rdf:type owl:Class ;
                 rdfs:subClassOf <https://w3id.org/pmd/co/Process> ;
                 rdfs:isDefinedBy <https://w3id.org/pmd/mo> ;
                 rdfs:label "Physical Process"@en ,
                            "Physikalischer Prozess"@de ;
                 <http://www.w3.org/2004/02/skos/core#definition> "A physical process refers to a sequence of events or interactions that occur in the physical world and can be described and analyzed based on the principles of physics. These processes involve the transformation of energy, matter, or both, and they often follow established laws and theories of physics. In particular, a physical process may just occur due to natural circumstances and does not necessarily have to be induced by human activities or interactions."@en ;
                 <https://w3id.org/pmd/co/definitionSource> "ChatGPT 3.5"@en .


###  https://w3id.org/pmd/mo/PixelSize
:PixelSize rdf:type owl:Class ;
           rdfs:subClassOf <https://w3id.org/pmd/co/ValueObject> ;
           rdfs:isDefinedBy <https://w3id.org/pmd/mo> ;
           rdfs:label "Pixel Size"@en ,
                      "Pixelgröße"@en ;
           <http://www.w3.org/2004/02/skos/core#definition> "Die Größe der einzelnen Pixel in einem digitalen Bild oder einer Anzeige."@de ,
                                                            "The size of individual pixels in a digital image or display."@en ;
           <https://w3id.org/pmd/co/definitionSource> "ChatGPT 3.5"@en .


###  https://w3id.org/pmd/mo/PolarizedLightMicroscope
:PolarizedLightMicroscope rdf:type owl:Class ;
                          rdfs:subClassOf :LightMicroscope ;
                          rdfs:isDefinedBy <https://w3id.org/pmd/mo> ;
                          rdfs:label "Polarisiertes Lichtmikroskop"@de ,
                                     "Polarized Light Microscope"@en ;
                          <http://www.w3.org/2004/02/skos/core#definition> "A microscope that uses polarized light to observe and analyze samples."@en ,
                                                                           "Ein Mikroskop, das polarisiertes Licht zur Beobachtung und Analyse von Proben verwendet."@de ;
                          <https://w3id.org/pmd/co/definitionSource> "ChatGPT 3.5"@en ;
                          :abbreviation "PLM"@en .


###  https://w3id.org/pmd/mo/PolarizedLightMicroscopy
:PolarizedLightMicroscopy rdf:type owl:Class ;
                          rdfs:subClassOf :LightMicroscopy ;
                          rdfs:isDefinedBy <https://w3id.org/pmd/mo> ;
                          rdfs:label "Polarisationslichtmikroskopie"@de ,
                                     "Polarized Light Microscopy"@en ;
                          <http://www.w3.org/2004/02/skos/core#definition> "Polarized Light Microscopy is a technique that uses polarized light to enhance the contrast and reveal structural information in transparent samples. Light waves vibrate in specific directions, and by using polarizers to control the orientation of light waves, polarized light microscopy can highlight birefringent materials, anisotropic structures, and stress patterns within samples. This technique is valuable for studying crystalline structures, fibers, and anisotropic materials."@en ;
                          <https://w3id.org/pmd/co/definitionSource> "ChatGPT 3.5"@en ;
                          :abbreviation "PLM"@en .


###  https://w3id.org/pmd/mo/PolePiece
:PolePiece rdf:type owl:Class ;
           rdfs:subClassOf <https://w3id.org/pmd/co/ProcessingNode> ;
           rdfs:comment "A given electron microscope is likely to have multiple pole pieces; however the term is commonly used to refer to the pole piece of the final optical element between the source  and the specimen."@en ,
                        "Ein bestimmtes Elektronenmikroskop hat wahrscheinlich mehrere Polschuhe; der Begriff wird jedoch üblicherweise für den Polschuh des letzten optischen Elements zwischen der Quelle und der Probe verwendet."@de ;
           rdfs:isDefinedBy <https://w3id.org/pmd/mo> ;
           rdfs:label "Pole Piece"@en ,
                      "Polschuh"@de ;
           <http://www.w3.org/2004/02/skos/core#definition> "Component of the electromagnetic lens which amplifies and shapes the magnetic field used to manipulate the beam."@en ,
                                                            "Komponente der elektromagnetischen Linse, die das zur Manipulation des Strahls verwendete Magnetfeld verstärkt und formt."@de ;
           <https://w3id.org/pmd/co/definitionSource> <https://codebase.helmholtz.cloud/em_glossary/em_glossary/-/blob/main/terms/pole_piece.yaml> ,
                                                      <https://en.wikipedia.org/wiki/Pole_piece> ,
                                                      <https://www.jeol.co.jp/en/words/emterms/search_result.html?keyword=polepiece> .


###  https://w3id.org/pmd/mo/PrimaryBeam
:PrimaryBeam rdf:type owl:Class ;
             rdfs:subClassOf :Beam ;
             rdfs:comment "Der Begriff wird bei Beugungsexperimenten üblicherweise verwendet, um den nicht gebeugten/nicht gestreuten Teil des Strahls nach der Probe zu beschreiben."@de ,
                          "The term is commonly used in diffraction experiments to describe the non-diffracted/non-scattered part of the beam after the specimen."@en ;
             rdfs:isDefinedBy <https://w3id.org/pmd/mo> ;
             rdfs:label "Primary Beam"@en ,
                        "Primärstrahl"@de ;
             <http://www.w3.org/2004/02/skos/core#definition> "A beam which is unaltered in terms of its direction after interaction with the specimen."@en ,
                                                              "Ein Strahl, der nach der Wechselwirkung mit dem Probekörper in seiner Richtung unverändert bleibt."@de ;
             <https://w3id.org/pmd/co/definitionSource> <https://codebase.helmholtz.cloud/em_glossary/em_glossary/-/blob/main/terms/primary-beam.yaml> ,
                                                        <https://www.iso.org/obp/ui/#iso:std:iso:15932:ed-1:v1:en> ,
                                                        <https://www.iso.org/obp/ui/#iso:std:iso:23833:ed-2:v1:en> .


###  https://w3id.org/pmd/mo/ProbeCurrent
:ProbeCurrent rdf:type owl:Class ;
              rdfs:subClassOf :Current ;
              rdfs:isDefinedBy <https://w3id.org/pmd/mo> ;
              rdfs:label "Probe Current"@en ,
                         "Sondenstrom"@de ;
              <http://www.w3.org/2004/02/skos/core#definition> "Electrical current which arrives at the specimen."@en ,
                                                               "Elektrischer Strom, der an der Probe ankommt."@de ;
              <https://w3id.org/pmd/co/definitionSource> <https://codebase.helmholtz.cloud/em_glossary/em_glossary/-/blob/main/terms/probe_current.yaml> .


###  https://w3id.org/pmd/mo/ProbeSize
:ProbeSize rdf:type owl:Class ;
           rdfs:subClassOf <https://w3id.org/pmd/co/ValueObject> ;
           rdfs:isDefinedBy <https://w3id.org/pmd/mo> ;
           rdfs:label "Probe Size"@en ,
                      "Sensorgröße"@de ;
           <http://www.w3.org/2004/02/skos/core#altLabel> "Messfühlergröße"@de ;
           <http://www.w3.org/2004/02/skos/core#definition> "Die Größe der Sonde oder des Strahls, die bei Mikroskopie- oder Spektroskopieverfahren verwendet werden."@de ,
                                                            "The size of the probe or beam used in microscopy or spectroscopy techniques."@en ;
           <https://w3id.org/pmd/co/definitionSource> "ChatGPT 3.5"@en .


###  https://w3id.org/pmd/mo/Reconstruction
:Reconstruction rdf:type owl:Class ;
                rdfs:subClassOf <https://w3id.org/pmd/co/AnalysingProcess> ;
                rdfs:isDefinedBy <https://w3id.org/pmd/mo> ;
                rdfs:label "Reconstruction"@en ,
                           "Rekonstruktion"@de ;
                <http://www.w3.org/2004/02/skos/core#definition> "Der Prozess der Erstellung eines dreidimensionalen Bildes oder Modells aus zweidimensionalen Daten."@de ,
                                                                 "The process of creating a three-dimensional image or model from two-dimensional data."@en ;
                <https://w3id.org/pmd/co/definitionSource> "ChatGPT 3.5"@en .


###  https://w3id.org/pmd/mo/Resolution
:Resolution rdf:type owl:Class ;
            rdfs:subClassOf <https://w3id.org/pmd/co/ValueObject> ;
            rdfs:isDefinedBy <https://w3id.org/pmd/mo> ;
            rdfs:label "Auflösung"@de ,
                       "Resolution"@en ;
            <http://www.w3.org/2004/02/skos/core#definition> "In various contexts, resolution refers to the degree of detail that can be discerned in an image, measurement, or other representation of an object or phenomenon."@en ,
                                                             "In verschiedenen Zusammenhängen bezieht sich die Auflösung auf den Grad der Detailgenauigkeit, die in einem Bild, einer Messung oder einer anderen Darstellung eines Objekts oder Phänomens erkennbar ist."@de ;
            <https://w3id.org/pmd/co/definitionSource> "ChatGPT 3.5"@en .


###  https://w3id.org/pmd/mo/ScanningElectronMicroscope
:ScanningElectronMicroscope rdf:type owl:Class ;
                            rdfs:subClassOf <https://w3id.org/pmd/co/ElectronMicroscope> ;
                            rdfs:isDefinedBy <https://w3id.org/pmd/mo> ;
                            rdfs:label "Rasterelektronenmikroskop"@de ,
                                       "Scanning Electron Microscope"@en ;
                            <http://www.w3.org/2004/02/skos/core#definition> "A microscope that produces images of a sample by scanning it with a focused beam of electrons."@en ,
                                                                             "Ein Mikroskop, das Bilder einer Probe erzeugt, indem es diese mit einem fokussierten Elektronenstrahl abtastet."@de ;
                            <https://w3id.org/pmd/co/definitionSource> "ChatGPT 3.5"@en ;
                            :abbreviation "REM"@de ,
                                          "SEM"@en .


###  https://w3id.org/pmd/mo/ScanningElectronMicroscopy
:ScanningElectronMicroscopy rdf:type owl:Class ;
                            rdfs:subClassOf <https://w3id.org/pmd/co/ElectronMicroscopy> ;
                            rdfs:isDefinedBy <https://w3id.org/pmd/mo> ;
                            rdfs:label "Rasterelektronenmikroskopie"@de ,
                                       "Scanning Electron Microscopy"@en ;
                            <http://www.w3.org/2004/02/skos/core#definition> "Scanning Electron Microscopy is a microscopy technique that uses a focused beam of electrons to scan the surface of a sample. The interaction of the electrons with the sample generates signals that provide information about the sample's topography, morphology, and composition."@en ;
                            <https://w3id.org/pmd/co/definitionSource> "ChatGPT 3.5"@en ;
                            :abbreviation "SEM"@en .


###  https://w3id.org/pmd/mo/ScanningProbeMicroscope
:ScanningProbeMicroscope rdf:type owl:Class ;
                         rdfs:subClassOf <https://w3id.org/pmd/co/ElectronMicroscope> ;
                         rdfs:isDefinedBy <https://w3id.org/pmd/mo> ;
                         rdfs:label "Rastersondenmikroskop"@de ,
                                    "Scanning Probe Microscope"@en ;
                         <http://www.w3.org/2004/02/skos/core#definition> "A type of microscope that images surfaces by scanning a probe over the sample."@en ,
                                                                          "Ein Mikroskoptyp, der Oberflächen abbildet, indem er eine Sonde über die Probe führt."@de ;
                         <https://w3id.org/pmd/co/definitionSource> "ChatGPT 3.5"@en .


###  https://w3id.org/pmd/mo/ScanningProbeMicroscopy
:ScanningProbeMicroscopy rdf:type owl:Class ;
                         rdfs:subClassOf <https://w3id.org/pmd/co/ElectronMicroscopy> ;
                         rdfs:isDefinedBy <https://w3id.org/pmd/mo> ;
                         rdfs:label "Rastersondenmikroskopie"@de ,
                                    "Scanning Probe Microscopy"@en ;
                         <http://www.w3.org/2004/02/skos/core#definition> "Scanning Probe Microscopy encompasses various techniques, such as Atomic Force Microscopy (AFM) and Scanning Tunneling Microscopy (STM), that use a sharp probe to scan a sample's surface. These techniques provide high-resolution images and information about surface properties on the nanometer scale."@en ;
                         <https://w3id.org/pmd/co/definitionSource> "ChatGPT 3.5"@en ;
                         :abbreviation "SPM"@en .


###  https://w3id.org/pmd/mo/ScanningTransmissionElectronMicroscope
:ScanningTransmissionElectronMicroscope rdf:type owl:Class ;
                                        rdfs:subClassOf :TransmissionElectronMicroscope ;
                                        rdfs:isDefinedBy <https://w3id.org/pmd/mo> ;
                                        rdfs:label "Rastertransmissionselektronenmikroskop"@de ,
                                                   "Scanning Transmission Electron Microscope"@en ;
                                        <http://www.w3.org/2004/02/skos/core#definition> "A type of transmission electron microscope where a focused electron beam is scanned across the sample."@en ,
                                                                                         "Eine Art von Transmissionselektronenmikroskop, bei dem ein fokussierter Elektronenstrahl über die Probe gescannt wird."@de ;
                                        <https://w3id.org/pmd/co/definitionSource> "ChatGPT 3.5"@en ;
                                        :abbreviation "STEM"@en .


###  https://w3id.org/pmd/mo/ScanningTransmissionElectronMicroscopy
:ScanningTransmissionElectronMicroscopy rdf:type owl:Class ;
                                        rdfs:subClassOf :TransmissionElectronMicroscopy ;
                                        rdfs:isDefinedBy <https://w3id.org/pmd/mo> ;
                                        rdfs:label "Rastertransmissionselektronenmikroskopie"@de ,
                                                   "Scanning Transmission Electron Microscopy"@en ;
                                        <http://www.w3.org/2004/02/skos/core#definition> "Scanning Transmission Electron Microscopy is a technique that combines the principles of scanning and transmission electron microscopy. It allows imaging and spectroscopy with high spatial resolution."@en ;
                                        <https://w3id.org/pmd/co/definitionSource> "ChatGPT 3.5"@en ;
                                        :abbreviation "STEM"@en .


###  https://w3id.org/pmd/mo/ScanningTransmissionElectronMicroscopy-ElectronEnergyLossSpectroscopy
:ScanningTransmissionElectronMicroscopy-ElectronEnergyLossSpectroscopy rdf:type owl:Class ;
                                                                       rdfs:subClassOf :ScanningTransmissionElectronMicroscopy ;
                                                                       rdfs:isDefinedBy <https://w3id.org/pmd/mo> ;
                                                                       rdfs:label "Rastertransmissionselektronenmikroskopie Elektronen-Energieverlust-Spektroskopie"@de ,
                                                                                  "Scanning Transmission Electron Microscopy Electron Energy Loss Spectroscopy"@en ;
                                                                       <http://www.w3.org/2004/02/skos/core#definition> "STEM-EELS combines STEM imaging with electron energy loss spectroscopy to provide information about the elemental composition and electronic structure of a sample at high spatial resolution."@en ;
                                                                       <https://w3id.org/pmd/co/definitionSource> "ChatGPT 3.5"@en ;
                                                                       :abbreviation "STEM-EELS"@en .


###  https://w3id.org/pmd/mo/ScanningTunnelingMicroscope
:ScanningTunnelingMicroscope rdf:type owl:Class ;
                             rdfs:subClassOf :ScanningProbeMicroscope ;
                             rdfs:isDefinedBy <https://w3id.org/pmd/mo> ;
                             rdfs:label "Rastertunnelmikroskop"@de ,
                                        "Scanning Tunneling Microscope"@en ;
                             <http://www.w3.org/2004/02/skos/core#definition> "A microscope that uses quantum tunneling to image surfaces at the atomic level."@en ,
                                                                              "Ein Mikroskop, das Quanten-Tunneling nutzt, um Oberflächen auf atomarer Ebene abzubilden."@de ;
                             <https://w3id.org/pmd/co/definitionSource> "ChatGPT 3.5"@en ;
                             :abbreviation "STM"@en .


###  https://w3id.org/pmd/mo/ScanningTunnelingMicroscopy
:ScanningTunnelingMicroscopy rdf:type owl:Class ;
                             rdfs:subClassOf :ScanningProbeMicroscopy ;
                             rdfs:isDefinedBy <https://w3id.org/pmd/mo> ;
                             rdfs:label "Rastertunnelmikroskopie"@de ,
                                        "Scanning Tunneling Microscopy"@en ;
                             <http://www.w3.org/2004/02/skos/core#definition> "Scanning Tunneling Microscopy is a technique that uses a conducting probe to measure the tunneling current between the probe and the sample's surface. It provides atomic-scale images of surfaces and is often used to study conductive materials."@en ;
                             <https://w3id.org/pmd/co/definitionSource> "ChatGPT 3.5"@en ;
                             :abbreviation "STM"@en .


###  https://w3id.org/pmd/mo/Scintillator
:Scintillator rdf:type owl:Class ;
              rdfs:subClassOf <https://w3id.org/pmd/co/ProcessingNode> ;
              rdfs:isDefinedBy <https://w3id.org/pmd/mo> ;
              rdfs:label "Scintillator"@en ,
                         "Szintillator"@de ;
              <http://www.w3.org/2004/02/skos/core#definition> "A material that emits light when it absorbs ionizing radiation."@en ,
                                                               "Ein Material, das Licht aussendet, wenn es ionisierende Strahlung absorbiert."@de ;
              <https://w3id.org/pmd/co/definitionSource> "ChatGPT 3.5"@en .


###  https://w3id.org/pmd/mo/SecondaryIonMassSpectrometry
:SecondaryIonMassSpectrometry rdf:type owl:Class ;
                              rdfs:subClassOf :Spectroscopy ;
                              rdfs:isDefinedBy <https://w3id.org/pmd/mo> ;
                              rdfs:label "Secondary Ion Mass Spectrometry"@en ,
                                         "Sekundärionen-Massenspektrometrie"@de ;
                              <http://www.w3.org/2004/02/skos/core#definition> """Secondary Ion Mass Spectrometry (SIMS) is an advanced analytical technique used to determine the elemental and isotopic composition of solid surfaces and thin films at a very high sensitivity and spatial resolution. It is widely employed in various scientific and industrial applications, including materials science, semiconductor research, and surface analysis.
In SIMS, a focused beam of high-energy primary ions is directed at a sample's surface. The impact of these primary ions causes the ejection of secondary ions from the sample's surface. These secondary ions are then extracted, mass-separated, and detected using a mass spectrometer. The mass spectrometer measures the mass-to-charge ratios of the secondary ions, providing information about the elemental and isotopic composition of the sample.
The sensitivity and spatial resolution of SIMS allow researchers to analyze very small areas, often down to the micrometer or nanometer scale. This makes SIMS particularly valuable for investigating surface composition, depth profiling of layered structures, and detecting trace elements in complex materials. The technique is non-destructive in its elemental analysis, which is beneficial for studying delicate samples or preserving valuable materials.
SIMS has applications in diverse fields, including materials characterization, semiconductor device analysis, biological and medical research, and geological studies. It provides essential information about the chemical composition, structure, and distribution of elements in complex samples, contributing to advancements in materials science and various technological developments."""@en ;
                              <https://w3id.org/pmd/co/definitionSource> "ChatGPT 3.5"@en ;
                              :abbreviation "SIMS"@en .


###  https://w3id.org/pmd/mo/SelectedAreaElectronDiffraction
:SelectedAreaElectronDiffraction rdf:type owl:Class ;
                                 rdfs:subClassOf :Diffraction ;
                                 rdfs:isDefinedBy <https://w3id.org/pmd/mo> ;
                                 rdfs:label "Elektronenbeugung ausgewählter Regionen"@de ,
                                            "Selected Area Electron Diffraction"@en ;
                                 <http://www.w3.org/2004/02/skos/core#definition> "Selected Area Electron Diffraction is a technique used in transmission electron microscopy (TEM) to study the crystallographic orientation of small regions within a sample. By selecting a specific area of the sample and directing an electron beam onto it, diffraction patterns are generated. These patterns offer insights into the sample's crystal structure and orientation."@en ;
                                 <https://w3id.org/pmd/co/definitionSource> "ChatGPT 3.5"@en ;
                                 :abbreviation "SAD"@en ,
                                               "SAED"@en .


###  https://w3id.org/pmd/mo/SiliconDriftDetector
:SiliconDriftDetector rdf:type owl:Class ;
                      rdfs:subClassOf <https://w3id.org/pmd/co/ProcessingNode> ;
                      rdfs:isDefinedBy <https://w3id.org/pmd/mo> ;
                      rdfs:label "Silicon Drift Detector"@en ,
                                 "Silizium-Driftdetektor"@de ;
                      <http://www.w3.org/2004/02/skos/core#definition> "A type of X-ray detector that offers high-speed performance and high energy resolution."@en ,
                                                                       "Eine Art Röntgendetektor, der Hochgeschwindigkeitsleistung und hohe Energieauflösung bietet."@de ;
                      <https://w3id.org/pmd/co/definitionSource> "ChatGPT 3.5"@en ;
                      :abbreviation "SDD"@en .


###  https://w3id.org/pmd/mo/SoftXRayEmissionSpectrometer
:SoftXRayEmissionSpectrometer rdf:type owl:Class ;
                              rdfs:subClassOf :Spectrometer ;
                              rdfs:isDefinedBy <https://w3id.org/pmd/mo> ;
                              rdfs:label "Röntgenemissionsspektrometer mit weicher Röntgenstrahlung"@de ,
                                         "Soft X-ray Emission Spectrometer"@en ;
                              <http://www.w3.org/2004/02/skos/core#definition> "An instrument used to analyze the emission of soft X-rays from a sample."@en ,
                                                                               "Ein Instrument zur Analyse der Emission weicher Röntgenstrahlen aus einer Probe."@de ;
                              <https://w3id.org/pmd/co/definitionSource> "ChatGPT 3.5"@en ;
                              :abbreviation "SXES"@en .


###  https://w3id.org/pmd/mo/Source
:Source rdf:type owl:Class ;
        rdfs:subClassOf <https://w3id.org/pmd/co/ProcessingNode> ;
        rdfs:comment "Die Art und Funktion der Quellen unterscheiden sich je nach Anwendungsfall und Gerät. Es gibt zwei Klassen von Emissionsquellen: thermionische Strahler (Glühfaden und LaB6) und Feldstrahler."@de ,
                     "The nature and the function of sources differ depending on application case and  instrument. There are two classes of emission sources, thermionic emitters (filament & LaB6) and field emitters."@en ;
        rdfs:isDefinedBy <https://w3id.org/pmd/mo> ;
        rdfs:label "Quelle"@de ,
                   "Source"@en ;
        <http://www.w3.org/2004/02/skos/core#definition> "A physical part of an electron or ion microscope from which the particles that form the beam are emitted."@en ,
                                                         "Ein physischer Teil eines Elektronen- oder Ionenmikroskops, aus dem die Teilchen, die den Strahl bilden, emittiert werden."@de ;
        <http://www.w3.org/2004/02/skos/core#example> """- Wolfram-Draht
- LaB_6-Kristall
- Wolfram-Kristall
- Flüssigmetall Gallium"""@de ,
                                                      """- tungsten wire
- LaB_6 crystal
- tungsten crystal
- liquid metal Gallium"""@en ;
        <https://w3id.org/pmd/co/definitionSource> <https://cmrf.research.uiowa.edu/scanning-electron-microscopy> ,
                                                   <https://codebase.helmholtz.cloud/em_glossary/em_glossary/-/blob/main/terms/source.yaml> .


###  https://w3id.org/pmd/mo/SpatialResolution
:SpatialResolution rdf:type owl:Class ;
                   rdfs:subClassOf :Resolution ;
                   rdfs:isDefinedBy <https://w3id.org/pmd/mo> ;
                   rdfs:label "Ortsauflösung"@de ,
                              "Spatial Resolution"@en ;
                   <http://www.w3.org/2004/02/skos/core#definition> "Die Fähigkeit eines Bildgebungssystems, feine Details in einem Objekt anzuzeigen. Sie bezieht sich auf das kleinste wahrnehmbare Detail in einem Bild."@de ,
                                                                    "The ability of an imaging system to discern fine details in an object. It refers to the smallest discernible detail in an image."@en ;
                   <https://w3id.org/pmd/co/definitionSource> "ChatGPT 3.5"@en .


###  https://w3id.org/pmd/mo/Spectrometer
:Spectrometer rdf:type owl:Class ;
              rdfs:subClassOf <https://w3id.org/pmd/co/ProcessingNode> ;
              rdfs:isDefinedBy <https://w3id.org/pmd/mo> ;
              rdfs:label "Spectrometer"@en ,
                         "Spektrometer"@de ;
              <http://www.w3.org/2004/02/skos/core#definition> "An instrument used to measure properties of light over a specific portion of the electromagnetic spectrum."@en ,
                                                               "Ein Instrument zur Messung der Eigenschaften von Licht in einem bestimmten Teil des elektromagnetischen Spektrums."@de ;
              <https://w3id.org/pmd/co/definitionSource> "ChatGPT 3.5"@en .


###  https://w3id.org/pmd/mo/Spectroscopy
:Spectroscopy rdf:type owl:Class ;
              rdfs:subClassOf <https://w3id.org/pmd/co/AnalysingProcess> ;
              rdfs:isDefinedBy <https://w3id.org/pmd/mo> ;
              <http://www.w3.org/2004/02/skos/core#altLabel> "Spectrometry"@en ,
                                                             "Spektrometrie"@de ;
              <http://www.w3.org/2004/02/skos/core#definition> "Spectroscopy is a scientific technique used to study and analyze the interaction of matter with electromagnetic radiation, such as light. It involves measuring the way in which different substances absorb, emit, or scatter light at various wavelengths or frequencies. By examining the spectrum of light emitted, absorbed, or transmitted by a sample, scientists can gain insights into its chemical composition, molecular structure, and physical properties. Spectroscopy is widely utilized in various fields, including chemistry, physics, astronomy, and biochemistry, to investigate the characteristics and behavior of materials at the atomic and molecular level."@en ;
              <http://www.w3.org/2004/02/skos/core#prefLabel> "Spectroscopy"@en ,
                                                              "Spektroskopie"@de ;
              <https://w3id.org/pmd/co/definitionSource> "ChatGPT 3.5"@en .


###  https://w3id.org/pmd/mo/SphericalAberration
:SphericalAberration rdf:type owl:Class ;
                     rdfs:subClassOf :Aberration ;
                     rdfs:isDefinedBy <https://w3id.org/pmd/mo> ;
                     rdfs:label "Spherical Aberration"@en ,
                                "Sphärische Aberration"@de ;
                     <http://www.w3.org/2004/02/skos/core#definition> "A type of optical aberration caused by deviations from the ideal spherical shape in lenses or mirrors."@en ,
                                                                      "Eine Art von optischer Aberration, die durch Abweichungen von der idealen sphärischen Form in Linsen oder Spiegeln verursacht wird."@de ;
                     <https://w3id.org/pmd/co/definitionSource> "ChatGPT 3.5"@en .


###  https://w3id.org/pmd/mo/SurfaceStructure
:SurfaceStructure rdf:type owl:Class ;
                  rdfs:subClassOf <https://w3id.org/pmd/co/Object> ;
                  rdfs:isDefinedBy <https://w3id.org/pmd/mo> ;
                  rdfs:label "Oberflächenstruktur"@de ,
                             "Surface Structure"@en ;
                  <http://www.w3.org/2004/02/skos/core#definition> "Die Anordnung und die Merkmale der äußersten Schicht eines Materials."@de ,
                                                                   "The arrangement and features of the outermost layer of a material."@en ;
                  <https://w3id.org/pmd/co/definitionSource> "ChatGPT 3.5"@en .


###  https://w3id.org/pmd/mo/TiltCorrection
:TiltCorrection rdf:type owl:Class ;
                rdfs:subClassOf <https://w3id.org/pmd/co/AnalysingProcess> ;
                rdfs:comment "Applied during acquisition to compensate for tilt. Tilt correction needs to be noted at data collection. Involves either stretching or compression along one direction / dimension of the scan area. An option in a GUI to switch on. Triggers a set of algorithms to apply stretching transformation on the image."@en ,
                             "Wird während der Erfassung angewendet, um die Neigung auszugleichen. Die Neigungskorrektur muss bei der Datenerfassung vermerkt werden. Dehnung oder Stauchung entlang einer Richtung/Dimension des Scanbereichs. Eine Option in einer grafischen Benutzeroberfläche zum Einschalten. Löst eine Reihe von Algorithmen aus, um eine Streckungstransformation auf das Bild anzuwenden."@de ;
                rdfs:isDefinedBy <https://w3id.org/pmd/mo> ;
                rdfs:label "Neigungskorrektur"@de ,
                           "Tilt Correction"@en ;
                <http://www.w3.org/2004/02/skos/core#definition> "An imaging setting which can be used during acquisition to correct perspective distortion when imaging a tilted surface or cross section."@en ,
                                                                 "Eine Bildgebungseinstellung, die während der Aufnahme verwendet werden kann, um perspektivische Verzerrungen bei der Abbildung einer geneigten Oberfläche oder eines Querschnitts zu korrigieren."@de ;
                <https://w3id.org/pmd/co/definitionSource> <https://codebase.helmholtz.cloud/em_glossary/em_glossary/-/blob/main/terms/tilt_correction.yaml> .


###  https://w3id.org/pmd/mo/TimeOfFlightSecondaryIonMassSpectrometry
:TimeOfFlightSecondaryIonMassSpectrometry rdf:type owl:Class ;
                                          rdfs:subClassOf :Spectroscopy ;
                                          rdfs:isDefinedBy <https://w3id.org/pmd/mo> ;
                                          rdfs:label "Flugzeit-Sekundärionen-Massenspektrometrie"@de ,
                                                     "Time Of Flight Secondary Ion Mass Spectrometry"@en ;
                                          <http://www.w3.org/2004/02/skos/core#definition> """Time-of-Flight Secondary Ion Mass Spectrometry (TOF-SIMS) is an advanced surface analysis technique used to determine the elemental and molecular composition of solid surfaces and thin films with high sensitivity and spatial resolution. It is employed in various scientific and industrial fields, including materials science, nanotechnology, biomedicine, and semiconductor research.
TOF-SIMS builds upon the principles of Secondary Ion Mass Spectrometry (SIMS), where a focused beam of high-energy primary ions is directed at a sample's surface, causing the ejection of secondary ions. In TOF-SIMS, the flight time of these secondary ions is measured as they travel through a field-free region and enter a time-of-flight mass spectrometer. The mass spectrometer measures the time taken by the ions to reach the detector, which is directly proportional to their mass-to-charge ratio.
By analyzing the flight times of the secondary ions, TOF-SIMS can determine the elemental, isotopic, and molecular composition of the sample's surface. It provides information about the presence of specific elements, chemical compounds, and molecular fragments, along with their spatial distribution. The high sensitivity of TOF-SIMS allows for the detection of trace elements and molecular species in complex samples.
TOF-SIMS is valuable for characterizing surfaces at the nanoscale, profiling layered structures, investigating organic and inorganic materials, and studying biological specimens. Its ability to provide detailed chemical information while maintaining spatial resolution makes it an essential tool for understanding surface properties and material interactions in a wide range of applications."""@en ;
                                          <https://w3id.org/pmd/co/definitionSource> "ChatGPT 3.5"@en ;
                                          :abbreviation "TOF-SIMS"@en .


###  https://w3id.org/pmd/mo/TomographicReconstruction
:TomographicReconstruction rdf:type owl:Class ;
                           rdfs:subClassOf :Reconstruction ;
                           rdfs:isDefinedBy <https://w3id.org/pmd/mo> ;
                           rdfs:label "Tomographic Reconstruction"@en ,
                                      "Tomographische Rekonstruktion"@de ;
                           <http://www.w3.org/2004/02/skos/core#definition> "Der Prozess der Rekonstruktion einer dreidimensionalen Struktur aus einer Reihe von zweidimensionalen Bildern, die aus verschiedenen Winkeln aufgenommen wurden."@de ,
                                                                            "The process of reconstructing a three-dimensional structure from a series of two-dimensional images taken at different angles."@en ;
                           <https://w3id.org/pmd/co/definitionSource> "ChatGPT 3.5"@en .


###  https://w3id.org/pmd/mo/TransmissionElectronAberrationCorrectedMicroscope
:TransmissionElectronAberrationCorrectedMicroscope rdf:type owl:Class ;
                                                   rdfs:subClassOf :TransmissionElectronMicroscope ;
                                                   rdfs:isDefinedBy <https://w3id.org/pmd/mo> ;
                                                   rdfs:label "Transmission Electron Aberration-corrected Microscope"@en ,
                                                              "Transmissionselektronen-Aberrations-korrigiertes Mikroskop"@de ;
                                                   <http://www.w3.org/2004/02/skos/core#definition> "A transmission electron microscope equipped with aberration correction to achieve high-resolution imaging."@en ,
                                                                                                    "Ein Transmissions-Elektronenmikroskop mit Aberrationskorrektur zur Erzielung hochauflösender Bilder."@de ;
                                                   <https://w3id.org/pmd/co/definitionSource> "ChatGPT 3.5"@en ;
                                                   :abbreviation "TEAM"@en .


###  https://w3id.org/pmd/mo/TransmissionElectronMicroscope
:TransmissionElectronMicroscope rdf:type owl:Class ;
                                rdfs:subClassOf <https://w3id.org/pmd/co/ElectronMicroscope> ;
                                rdfs:isDefinedBy <https://w3id.org/pmd/mo> ;
                                rdfs:label "Transmission Electron Microscope"@en ,
                                           "Transmissionelektronenmikroskop"@de ;
                                <http://www.w3.org/2004/02/skos/core#definition> "A microscope that transmits a beam of electrons through a specimen, forming an image."@en ,
                                                                                 "Ein Mikroskop, das einen Elektronenstrahl durch eine Probe sendet und ein Bild erzeugt."@de ;
                                <https://w3id.org/pmd/co/definitionSource> "ChatGPT 3.5"@en ;
                                :abbreviation "TEM" .


###  https://w3id.org/pmd/mo/TransmissionElectronMicroscopy
:TransmissionElectronMicroscopy rdf:type owl:Class ;
                                rdfs:subClassOf <https://w3id.org/pmd/co/ElectronMicroscopy> ;
                                rdfs:isDefinedBy <https://w3id.org/pmd/mo> ;
                                <http://www.w3.org/2004/02/skos/core#definition> "Transmission Electron Microscopy is a microscopy technique that involves transmitting a beam of electrons through a thin sample to create high-resolution images. It is used to study the internal structure and morphology of materials at the nanometer scale."@en ;
                                <https://w3id.org/pmd/co/definitionSource> "ChatGPT 3.5"@en ;
                                :abbreviation "TEM"@en .


###  https://w3id.org/pmd/mo/Voltage
:Voltage rdf:type owl:Class ;
         rdfs:subClassOf <https://w3id.org/pmd/co/ValueObject> ;
         rdfs:isDefinedBy <https://w3id.org/pmd/mo> ;
         rdfs:label "Spannung"@de ,
                    "Voltage"@en ;
         <http://www.w3.org/2004/02/skos/core#altLabel> "Stromspannung"@de ;
         <http://www.w3.org/2004/02/skos/core#definition> """Die Spannung, auch elektrische Potentialdifferenz, ist ein Maß für die elektrische potentielle Energie pro Ladungseinheit in einem elektrischen Stromkreis. Sie ist die Kraft, die den elektrischen Strom durch einen Leiter treibt. 

Hinweis: Die Spannung wird in Volt (V) gemessen und stellt die potenzielle Energiedifferenz zwischen zwei Punkten in einem Stromkreis dar. Je höher die Spannung ist, desto größer ist die Kraft, die die elektrischen Ladungen antreibt, und desto höher ist folglich auch das Potenzial für einen Stromfluss."""@de ,
                                                          """Voltage, also known as electric potential difference, is a measure of the electric potential energy per unit charge in an electrical circuit. It is the force or pressure that drives electric current through a conductor. 

Note: Voltage is measured in volts (V), and it represents the potential energy difference between two points in a circuit. The higher the voltage, the greater the force pushing the electric charges, and consequently, the higher the potential for current to flow."""@en ;
         <https://w3id.org/pmd/co/definitionSource> "ChatGPT 3.5"@en .


###  https://w3id.org/pmd/mo/Volume
:Volume rdf:type owl:Class ;
        rdfs:subClassOf <https://w3id.org/pmd/co/ValueObject> ;
        rdfs:isDefinedBy <https://w3id.org/pmd/mo> ;
        rdfs:label "Volume"@en ,
                   "Volumen"@de ;
        <http://www.w3.org/2004/02/skos/core#definition> "Die Menge an Raum, die ein Stoff oder Gegenstand einnimmt."@de ,
                                                         "The amount of space that a substance or object occupies."@en ;
        <https://w3id.org/pmd/co/definitionSource> "ChatGPT 3.5"@en .


###  https://w3id.org/pmd/mo/WaitTime
:WaitTime rdf:type owl:Class ;
          rdfs:subClassOf <https://w3id.org/pmd/co/Duration> ;
          rdfs:comment "Wait time can happen for multiple reasons. For example, the time period until a detector is ready (e.g. eds detector is cooled down. The time period until the specimen has reached the desired state for a measurement (e.g. in-situ heating/cooling). The time period until the machine has reached the desired state (e.g. switching from high vacuum to low vacuum mode in a variable pressure SEM). Frame flyback time may also be considered a wait time."@en ,
                       "Wartezeiten können aus verschiedenen Gründen entstehen. Zum Beispiel die Zeitspanne, bis ein Detektor bereit ist (z. B. der Detektor wird abgekühlt). Die Zeitspanne, bis die Probe den gewünschten Zustand für eine Messung erreicht hat (z. B. In-situ-Erwärmung/Kühlung). Die Zeitspanne, bis das Gerät den gewünschten Zustand erreicht hat (z. B. Umschalten von Hochvakuum auf Niedrigvakuum in einem REM mit variablem Druck). Die Rahmenrücklaufzeit kann auch als Wartezeit betrachtet werden."@de ;
          rdfs:isDefinedBy <https://w3id.org/pmd/mo> ;
          rdfs:label "Wait Time"@en ,
                     "Wartezeit"@de ;
          <http://www.w3.org/2004/02/skos/core#altLabel> "Abgelaufene Zeit"@de ,
                                                         "Elapsed Time"@en ;
          <http://www.w3.org/2004/02/skos/core#definition> "Time period in which no data are acquired."@en ,
                                                           "Zeitspanne, in der keine Daten erfasst werden."@de ;
          <https://w3id.org/pmd/co/definitionSource> <https://codebase.helmholtz.cloud/em_glossary/em_glossary/-/blob/main/terms/wait_time.yaml> .


###  https://w3id.org/pmd/mo/WorkingDistance
:WorkingDistance rdf:type owl:Class ;
                 rdfs:subClassOf <https://w3id.org/pmd/co/Distance> ;
                 rdfs:comment "Der Arbeitsabstand ist eine Eigenschaft des optischen Systems und als solche unabhängig von der Position der Probe. Bei regulärem Betrieb, z. B. von REM und STEM, befindet sich der hier erwähnte Fokuspunkt in unmittelbarer Nähe der Probenoberfläche. Die übliche Einheit für den Arbeitsabstand ist Millimeter. Der Begriff wird häufig in der Rasterelektronenmikroskopie und der Rasterionenmikroskopie verwendet. In modernen Rasterelektronenmikroskopen und Mikroskopen mit fokussiertem Ionenstrahl wird er auf der Benutzeroberfläche angezeigt und ist ein kalibrierter Wert, der auf der endgültigen Linsenanregung basiert. Aus praktischen Gründen bezieht er sich in der Regel auf das untere Ende der Säule und nicht auf die Linse, da dies dem Benutzer einen Hinweis darauf gibt, wie viel Platz zwischen der Säule und der Probenoberfläche ist, wenn letztere im Fokus ist. Im Allgemeinen verbessert ein kurzer Arbeitsabstand die Auflösung und die Signalerfassung bei In-Säulen-Detektoren."@de ,
                              "Working distance is a property of the optical system and as such independent of the position of  the specimen. During regular operation, e.g. of SEM & STEM, the here mentioned point of focus will be in direct vicinity of the specimen surface. Typically, the unit used for expressing the working distance is millimetre. The term is frequently used in scanning electron microscopy & scanning ion microscopy. In modern SEM and focused ion beam microscopes it is displayed in the user interface and it's a calibrated value based on the final lens excitation. For practical reasons it commonly refers to the lower end of the column instead of the lens as this gives the user an indication how much space  there is between the column and the sample surface when the latter is in focus. In general, a short working distance improves resolution and signal collection for in-column detectors."@en ;
                 rdfs:isDefinedBy <https://w3id.org/pmd/mo> ;
                 rdfs:label "Arbeitsabstand"@de ,
                            "Working Distance"@en ;
                 <http://www.w3.org/2004/02/skos/core#definition> "Abstand, der entlang der optischen Achse innerhalb der Säule von (1) dem unteren Ende des letzten optischen Elements zwischen der Quelle und dem Probentisch bis (2) dem Punkt, an dem der Strahl fokussiert wird, bestimmt wird."@de ,
                                                                  "Distance which is determined along the optical axis within the column from (1) the lower end of the final optical element between the source and the  specimen stage; to (2) the point where the beam is focused."@en ;
                 <https://w3id.org/pmd/co/definitionSource> <https://codebase.helmholtz.cloud/em_glossary/em_glossary/-/blob/main/terms/working_distance.yaml> ,
                                                            <https://www.globalsino.com/EM/page4586.html> .


###  https://w3id.org/pmd/mo/XRayAbsorptionNearEdgeSpectroscopy
:XRayAbsorptionNearEdgeSpectroscopy rdf:type owl:Class ;
                                    rdfs:subClassOf :Spectroscopy ;
                                    rdfs:isDefinedBy <https://w3id.org/pmd/mo> ;
                                    rdfs:label "Röntgenabsorptionsspektroskopie im Nahbereich"@de ,
                                               "X-ray Absorption Near Edge Spectroscopy"@en ;
                                    <http://www.w3.org/2004/02/skos/core#definition> """X-ray Absorption Near Edge Spectroscopy (XANES) is a specialized technique used in the field of materials science and spectroscopy to study the electronic and structural properties of materials. It focuses on the X-ray absorption spectra of atoms within a sample, particularly the region just above the absorption edge of an element's X-ray absorption spectrum.
In XANES, a sample is irradiated with X-rays, typically generated by a synchrotron radiation source. These X-rays are tuned to specific energy levels corresponding to the absorption edges of the elements of interest in the sample. As the X-rays are absorbed by the sample, the energy levels of the atoms are altered, leading to various transitions in their electron configurations. The resulting X-ray absorption spectrum is measured, specifically targeting the energies just above the absorption edge.
XANES provides information about the electronic structure of the atoms within the sample, including the oxidation state, chemical bonding, and local environment of the absorbing element. The fine details of the XANES spectrum offer insights into the atomic and molecular interactions, as well as the coordination and symmetry of atoms in different chemical environments.
This technique is widely used in various scientific fields, including chemistry, solid-state physics, and materials science. XANES helps researchers understand the properties and behavior of materials at the atomic level, making it an invaluable tool for investigating the characteristics of complex materials, catalysts, minerals, and biomolecules."""@en ;
                                    <https://w3id.org/pmd/co/definitionSource> "ChatGPT 3.5"@en ;
                                    :abbreviation "XANES"@en .


###  https://w3id.org/pmd/mo/XRayAbsorptionSpectroscopy
:XRayAbsorptionSpectroscopy rdf:type owl:Class ;
                            rdfs:subClassOf :XRayMapping ;
                            rdfs:isDefinedBy <https://w3id.org/pmd/mo> ;
                            rdfs:label "Röntgenabsorptionsspektroskopie"@de ,
                                       "X-ray Absorption Spectroscopy"@en ;
                            <http://www.w3.org/2004/02/skos/core#definition> "X-ray Absorption Spectroscopy is a technique used to study the electronic and local structural properties of materials by analyzing the absorption of X-rays. It involves measuring how X-rays are absorbed by a sample at various energies, providing insights into the electronic states and chemical environments of specific elements."@en ;
                            <https://w3id.org/pmd/co/definitionSource> "ChatGPT 3.5"@en ;
                            :abbreviation "XAS"@en .


###  https://w3id.org/pmd/mo/XRayAnalysis
:XRayAnalysis rdf:type owl:Class ;
              rdfs:subClassOf <https://w3id.org/pmd/co/AnalysingProcess> ;
              rdfs:isDefinedBy <https://w3id.org/pmd/mo> ;
              rdfs:label "Röntgenanalyse"@de ,
                         "X-ray Analysis"@en ;
              <http://www.w3.org/2004/02/skos/core#definition> "X-ray analysis is a technique used to investigate the composition and structure of materials by exposing them to X-rays. When X-rays interact with a material, they can be absorbed, scattered, or diffracted in ways that provide information about the material's internal arrangement of atoms and its elemental composition."@en ;
              <https://w3id.org/pmd/co/definitionSource> "ChatGPT 3.5"@en .


###  https://w3id.org/pmd/mo/XRayDiffraction
:XRayDiffraction rdf:type owl:Class ;
                 rdfs:subClassOf :Diffraction ;
                 rdfs:isDefinedBy <https://w3id.org/pmd/mo> ;
                 rdfs:label "X-ray Diffraction"@en ;
                 <http://www.w3.org/2004/02/skos/core#altLabel> "Röntgenstrahlbeugung"@de ;
                 <http://www.w3.org/2004/02/skos/core#definition> "X-ray Diffraction is a technique that utilizes the diffraction of X-rays by crystals to determine their atomic arrangement and lattice structure. X-ray diffraction patterns are produced when X-rays strike a crystalline sample, and the resulting pattern provides information about the arrangement of atoms in the crystal lattice."@en ;
                 <http://www.w3.org/2004/02/skos/core#prefLabel> "Röntgenbeugung"@de ;
                 <https://w3id.org/pmd/co/definitionSource> "ChatGPT 3.5"@en ;
                 :abbreviation "XRD"@en .


###  https://w3id.org/pmd/mo/XRayFluorescence
:XRayFluorescence rdf:type owl:Class ;
                  rdfs:subClassOf :XRayMapping ;
                  rdfs:isDefinedBy <https://w3id.org/pmd/mo> ;
                  rdfs:label "Röntgenfluoreszenz"@de ,
                             "X-ray Fluorescence"@en ;
                  <http://www.w3.org/2004/02/skos/core#definition> "X-ray Fluorescence is a method used to determine the elemental composition of a sample by analyzing the X-rays emitted when the sample is exposed to high-energy X-rays. The X-rays emitted are characteristic of the elements present, allowing for quantitative analysis of the sample's elemental composition."@en ;
                  <https://w3id.org/pmd/co/definitionSource> "ChatGPT 3.5"@en ;
                  :abbreviation "XRF"@en .


###  https://w3id.org/pmd/mo/XRayMapping
:XRayMapping rdf:type owl:Class ;
             rdfs:subClassOf :XRayAnalysis ;
             rdfs:isDefinedBy <https://w3id.org/pmd/mo> ;
             rdfs:label "Röntgen-Mapping"@de ,
                        "X-ray Mapping"@en ;
             <http://www.w3.org/2004/02/skos/core#definition> "X-ray mapping is a process that involves generating spatially resolved images of the distribution of specific elements within a sample. By collecting X-ray signals emitted or scattered from a sample at different points, an elemental map can be created, showing the varying concentrations of elements across the sample's surface."@en ;
             <https://w3id.org/pmd/co/definitionSource> "ChatGPT 3.5"@en .


###  https://w3id.org/pmd/mo/XRayMicroanalysis
:XRayMicroanalysis rdf:type owl:Class ;
                   rdfs:subClassOf :XRayAnalysis ;
                   rdfs:isDefinedBy <https://w3id.org/pmd/mo> ;
                   rdfs:label "Röntgen-Mikroanalyse"@de ,
                              "X-ray Microanalysis"@en ;
                   <http://www.w3.org/2004/02/skos/core#definition> "X-ray Microanalysis is a technique that combines microscopy and X-ray analysis to study the elemental composition of small regions within a sample. It involves focusing an electron or X-ray beam on a specific area of the sample and measuring the X-rays emitted from that area to determine the elemental composition."@en ;
                   <https://w3id.org/pmd/co/definitionSource> "ChatGPT 3.5"@en .


###  https://w3id.org/pmd/mo/XRayPhotoelectronSpectroscopy
:XRayPhotoelectronSpectroscopy rdf:type owl:Class ;
                               rdfs:subClassOf :XRayMapping ;
                               rdfs:isDefinedBy <https://w3id.org/pmd/mo> ;
                               rdfs:label "Röntgenphotoelektronenspektroskopie"@de ,
                                          "X-ray Photoelectron Spectroscopy"@en ;
                               <http://www.w3.org/2004/02/skos/core#definition> "X-ray Photoelectron Spectroscopy, also known as Electron Spectroscopy for Chemical Analysis (ESCA), is a technique used to study the surface chemistry of materials. XPS involves bombarding a sample's surface with X-rays to emit photoelectrons, which are then analyzed to determine the elemental composition and chemical states of the elements on the surface."@en ;
                               <https://w3id.org/pmd/co/definitionSource> "ChatGPT 3.5"@en ;
                               :abbreviation "XPS"@en .


###  https://w3id.org/pmd/mo/3DReconstruction
<https://w3id.org/pmd/mo/3DReconstruction> rdf:type owl:Class ;
                                           rdfs:subClassOf :Reconstruction ;
                                           rdfs:isDefinedBy <https://w3id.org/pmd/mo> ;
                                           rdfs:label "Dreidimensionale Rekonstruktion"@de ,
                                                      "Three dimensional reconstruction"@en ;
                                           <http://www.w3.org/2004/02/skos/core#definition> "Der Prozess der Erstellung einer dreidimensionalen Darstellung eines Objekts oder einer Szene aus zweidimensionalen Bildern oder Daten."@de ,
                                                                                            "The process of creating a three-dimensional representation of an object or scene from two-dimensional images or data."@en ;
                                           <https://w3id.org/pmd/co/definitionSource> "ChatGPT 3.5"@en .


###  https://w3id.org/pmd/mo/4D-ScanningTransmissionElectronMicroscopy
<https://w3id.org/pmd/mo/4D-ScanningTransmissionElectronMicroscopy> rdf:type owl:Class ;
                                                                    rdfs:subClassOf :ScanningTransmissionElectronMicroscopy ;
                                                                    rdfs:isDefinedBy <https://w3id.org/pmd/mo> ;
                                                                    rdfs:label "4D Scanning Transmission Electron Microscopy"@en ,
                                                                               "4D-Rastertransmissionselektronenmikroskopie"@de ;
                                                                    <http://www.w3.org/2004/02/skos/core#definition> "4D-STEM is a technique that adds an additional dimension of information, time, to STEM imaging, allowing the study of dynamic processes in materials at high spatial and temporal resolutions."@en ;
                                                                    <https://w3id.org/pmd/co/definitionSource> "ChatGPT 3.5"@en ;
                                                                    :abbreviation "4D-STEM"@en .


###  Generated by the OWL API (version 4.5.9.2019-02-01T07:24:44Z) https://github.com/owlcs/owlapi
